Prove compilation of expressions with couple of cheats

pancake/proofs/crep_to_loopProofScript.sml
@@ -18,76 +18,73 @@ Datatype:
      vmax : num|>
 End
 
-
-Definition comp_assigns_def:
-  (comp_assigns f ctxt [] =  Skip) /\
-  (comp_assigns f ctxt (e::es) =
-   Seq (f ctxt e)
-       (comp_assigns f (ctxt with vmax := ctxt.vmax + 1) es))
+Definition find_var_def:
+  find_var ct v =
+   case FLOOKUP ct.vars v of
+    | SOME n => n
+    | NONE => 0
 End
 
-
-
-(*
-Definition comp_assigns_def:
-  (comp_assigns f m re [] =  Skip) /\
-  (comp_assigns f m re (e::es) =
-   Seq (Seq (f e) (Assign m re))
-       (comp_assigns f (m+1) re es))
+Definition find_lab_def:
+  find_lab ct f =
+   case FLOOKUP ct.funcs f of
+    | SOME (n, _) => n
+    | NONE => 0
 End
-*)
 
-Definition load_exps_def:
-  load_exps n m  = MAP Var (GENLIST (λx. n + x) m)
+Definition nested_seq_def:
+  (nested_seq [] = (Skip:'a loopLang$prog)) /\
+  (nested_seq (e::es) = Seq e (nested_seq es))
+End
+
+Definition prog_if_def:
+  prog_if cmp p q e e' n m l =
+   p ++ q ++ [
+    Assign n e; Assign m e';
+    If cmp n (Reg m)
+    (Assign n (Const 1w)) (Assign n (Const 0w)) (insert n () l)]
 End
 
 Definition compile_exp_def:
-  (compile_exp ctxt ((Const c):'a crepLang$exp) =
-   Assign (ctxt.vmax + 1) ((Const c): 'a loopLang$exp)) /\
-  (compile_exp ctxt (Var vname) = Assign (ctxt.vmax + 1)
-   (case FLOOKUP ctxt.vars vname of
-     | SOME n => Var n
-     | NONE => Var 0)) /\
-  (compile_exp ctxt (Label fname) = LocValue (ctxt.vmax + 1)
-   (case FLOOKUP ctxt.funcs fname of
-     | SOME (n, _) => n
-     | NONE => 0)) /\
-  (compile_exp ctxt (Load adr) =
-   Seq (compile_exp ctxt adr)
-       (Assign (ctxt.vmax + 1) (Load (Var (ctxt.vmax + 1))))) /\
-  (compile_exp ctxt (LoadByte adr) =
-   Seq (compile_exp ctxt adr)
-       (LoadByte (ctxt.vmax + 1) 0w (ctxt.vmax + 1))) /\
-  (compile_exp ctxt (LoadGlob gadr) = Assign (ctxt.vmax + 1) (Lookup gadr)) /\
-  (compile_exp ctxt (Op bop es) =
-   Seq (comp_assigns (λc e. compile_exp c e) ctxt es)
-       (Assign (ctxt.vmax + 1) (Op bop (load_exps (ctxt.vmax + 1) (LENGTH es))))) /\
+  (compile_exp ctxt tmp l ((Const c):'a crepLang$exp) = ([], Const c, tmp, l)) /\
+  (compile_exp ctxt tmp l (Var v) = ([], Var (find_var ctxt v), tmp, l)) /\
+  (compile_exp ctxt tmp l (Label f) = ([LocValue tmp (find_lab ctxt f)], Var tmp, tmp + 1, insert tmp () l)) /\
+  (compile_exp ctxt tmp l (Load ad) =
+   let (p, le, tmp, l) = compile_exp ctxt tmp l ad in (p, Load le, tmp, l)) /\
+  (compile_exp ctxt tmp l (LoadByte ad) =
+   let (p, le, tmp, l) = compile_exp ctxt tmp l ad in
+    (p ++ [Assign tmp le; LoadByte tmp 0w tmp], Var tmp, tmp + 1, insert tmp () l)) /\
+  (compile_exp ctxt tmp l (LoadGlob gadr) = ([], Lookup gadr, tmp, l)) /\
+  (compile_exp ctxt tmp l (Op bop es) =
+   let (p, les, tmp, l) = compile_exps ctxt tmp l es in
+   (p, Op bop les, tmp, l)) /\
+  (compile_exp ctxt tmp l (Cmp cmp e e') =
+   let (p, le, tmp, l) = compile_exp ctxt tmp l e in
+   let (p', le', tmp', l) = compile_exp ctxt tmp l e' in
+    (prog_if cmp p p' le le' (tmp' + 1) (tmp' + 2) l, Var (tmp' + 1), tmp' + 3, insert (tmp' + 1) () l)) /\
+  (compile_exp ctxt tmp l (Shift sh e n) =
+   let (p, le, tmp, l) = compile_exp ctxt tmp l e in (p, Shift sh le n, tmp, l)) /\
 
-
-(*  (compile_exp ctxt (Op bop es) =
-   Seq (comp_assigns (compile_exp ctxt) (ctxt.vmax + 2) (Var (ctxt.vmax + 1)) es)
-       (Assign (ctxt.vmax + 1) (Op bop (load_exps (ctxt.vmax + 2) (LENGTH es))))) /\ *)
-  (compile_exp ctxt (Cmp cmp e e') =
-   Seq (Seq (compile_exp ctxt e) (compile_exp (ctxt with vmax := ctxt.vmax + 1) e'))
-        (If cmp (ctxt.vmax + 1) (Reg (ctxt.vmax + 2))
-           (Assign (ctxt.vmax + 1) (Const 1w)) (Assign (ctxt.vmax + 1) (Const 0w)) LN)) /\
-  (compile_exp ctxt (Shift sh e n) =
-   Seq (compile_exp ctxt e)
-   (Assign (ctxt.vmax + 1) (Shift sh (Var (ctxt.vmax + 1)) n)))
+  (compile_exps ctxt tmp l cps = (* to generate ind thm *)
+   case cps of
+   | [] => ([], [], tmp, l)
+   | e::es =>
+     let (p, le, tmp, l) = compile_exp ctxt tmp l e in
+      let (p1, les, tmp, l) = compile_exps ctxt tmp l es in
+      (p ++ p1, le::les, tmp, l))
 Termination
   cheat
 End
 
-
-
 Definition compile_prog_def:
-  (compile_prog _ (Skip:'a crepLang$prog) = (Skip:'a loopLang$prog)) /\
-  (compile_prog _ (Dec v e p) = ARB) /\
-  (compile_prog ctxt (Assign v e) =
-    Seq (compile_exp ctxt e)
-        (Assign v (Var (ctxt.vmax + 1))))
+  (compile_prog _ l (Skip:'a crepLang$prog) = (Skip:'a loopLang$prog, l)) /\
+  (compile_prog ctxt l (Assign v e) =
+   case FLOOKUP ctxt.vars v of
+    | SOME n =>
+      let (p,le,tmp, l) = compile_exp ctxt (ctxt.vmax + 1) l e in
+       (nested_seq (p ++ [Assign n le]), l)
+    | NONE => (Skip,l))
 End
-
 
 (* state relation *)
 
@@ -112,7 +109,7 @@ Definition wlab_wloc_def:
   (wlab_wloc ctxt (Label fname) =
    case FLOOKUP ctxt.funcs fname of
     | SOME (n, _) =>  Loc n 0
-    | NONE =>  Loc 0 0)
+    | NONE =>  Loc 0 0)  (* impossible *)
 End
 
 Definition mem_rel_def:
@@ -152,10 +149,10 @@ Definition code_rel_def:
    distinct_funcs ctxt.funcs /\
    (∀f ns prog.
      FLOOKUP s_code f = SOME (ns, prog) ==>
-     ?loc args. FLOOKUP ctxt.funcs f = SOME (loc, args) /\
+     ?loc args l. FLOOKUP ctxt.funcs f = SOME (loc, args) /\
        LENGTH ns = LENGTH args /\
        let nctxt = ctxt_fc ctxt.funcs ns args  in
-       lookup loc t_code = SOME (ns, compile_prog nctxt prog))
+       lookup loc t_code = SOME (ns, FST (compile_prog nctxt l prog)))
 End
 
 Definition excp_rel_def:
@@ -176,47 +173,32 @@ Definition distinct_vars_def:
        n = m ==> x = y)
 End
 
-
 Definition locals_rel_def:
-  locals_rel ctxt (s_locals:num |-> 'a word_lab) t_locals <=>
-  distinct_vars ctxt.vars /\ ctxt_max ctxt.vmax ctxt.vars /\
+  locals_rel ctxt (l:sptree$num_set) (s_locals:num |-> 'a word_lab) t_locals <=>
+  distinct_vars ctxt.vars /\ ctxt_max ctxt.vmax ctxt.vars /\ domain l ⊆ domain t_locals /\
   ∀vname v.
     FLOOKUP s_locals vname = SOME v ==>
-    ∃n v'. FLOOKUP ctxt.vars vname = SOME n ∧
+    ∃n v'. FLOOKUP ctxt.vars vname = SOME n ∧ n ∈ domain l ∧ (* remove that later *)
     lookup n t_locals = SOME v' ∧ wlab_wloc ctxt v = v'
 End
 
-val goal =
-  ``λ(prog, s). ∀res s1 t ctxt.
-      evaluate (prog,s) = (res,s1) ∧ res ≠ SOME Error ∧
-      state_rel s t ∧ code_rel ctxt s.code t.code /\
-      locals_rel ctxt s.locals t.locals ⇒
-      ∃res1 t1. evaluate (compile_prog ctxt prog,t) = (res1,t1) /\
-      state_rel s1 t1 ∧ code_rel ctxt s1.code t1.code /\
-      case res of
-       | NONE => res1 = NONE /\ locals_rel ctxt s1.locals t1.locals
-       | SOME _ => ARB``
-
-local
-  val ind_thm = crepSemTheory.evaluate_ind
-    |> ISPEC goal
-    |> CONV_RULE (DEPTH_CONV PairRules.PBETA_CONV) |> REWRITE_RULE [];
-  fun list_dest_conj tm = if not (is_conj tm) then [tm] else let
-    val (c1,c2) = dest_conj tm in list_dest_conj c1 @ list_dest_conj c2 end
-  val ind_goals = ind_thm |> concl |> dest_imp |> fst |> list_dest_conj
-in
-  fun get_goal s = first (can (find_term (can (match_term (Term [QUOTE s]))))) ind_goals
-  fun compile_prog_tm () = ind_thm |> concl |> rand
-  fun the_ind_thm () = ind_thm
-end
+Theorem state_rel_intro:
+  state_rel ^s (t:('a,'ffi) loopSem$state) <=>
+  s.memaddrs = t.mdomain ∧
+  s.clock = t.clock ∧
+  s.be = t.be ∧
+  s.ffi = t.ffi
+Proof
+  rw [state_rel_def]
+QED
 
 
 Theorem locals_rel_intro:
-  locals_rel ctxt (s_locals:num |-> 'a word_lab) t_locals ==>
-  distinct_vars ctxt.vars /\ ctxt_max ctxt.vmax ctxt.vars /\
+  locals_rel ctxt l (s_locals:num |-> 'a word_lab) t_locals ==>
+  distinct_vars ctxt.vars /\ ctxt_max ctxt.vmax ctxt.vars /\ domain l ⊆ domain t_locals /\
   ∀vname v.
     FLOOKUP s_locals vname = SOME v ==>
-    ∃n v'. FLOOKUP ctxt.vars vname = SOME n ∧
+    ∃n v'. FLOOKUP ctxt.vars vname = SOME n ∧ n ∈ domain l ∧
     lookup n t_locals = SOME v' ∧ wlab_wloc ctxt v = v'
 Proof
   rw [locals_rel_def]
@@ -227,10 +209,10 @@ Theorem code_rel_intro:
    distinct_funcs ctxt.funcs /\
    (∀f ns prog.
      FLOOKUP s_code f = SOME (ns, prog) ==>
-     ?loc args. FLOOKUP ctxt.funcs f = SOME (loc, args) /\
+     ?loc args l . FLOOKUP ctxt.funcs f = SOME (loc, args) /\
        LENGTH ns = LENGTH args /\
        let nctxt = ctxt_fc ctxt.funcs ns args  in
-       lookup loc t_code = SOME (ns, compile_prog nctxt prog))
+       lookup loc t_code = SOME (ns, FST (compile_prog nctxt l prog)))
 Proof
   rw [code_rel_def]
 QED
@@ -255,6 +237,3850 @@ Theorem globals_rel_intro:
 Proof
   rw [globals_rel_def]
 QED
+
+
+Theorem evaluate_nested_seq_cases:
+  (!p q s st t.
+    evaluate (nested_seq (p ++ q), s) = (NONE, t) /\
+    evaluate (nested_seq p,s) = (NONE,st) ==>
+    evaluate (nested_seq q,st) = (NONE,t)) /\
+  (!p s st q.
+    evaluate (nested_seq p, s) = (NONE, st) ==>
+    evaluate (nested_seq (p ++ q), s) =  evaluate (nested_seq q, st)) /\
+  (!p s res st q.
+    evaluate (nested_seq p, s) = (res, st) /\
+    res <> NONE ==>
+    evaluate (nested_seq (p ++ q), s) =  evaluate (nested_seq p, s))
+Proof
+  rpt conj_tac >>
+  Induct >> rw []
+  >- fs [nested_seq_def, evaluate_def] >>
+  fs [nested_seq_def, evaluate_def] >>
+  pairarg_tac >> fs [] >>
+  FULL_CASE_TAC >> fs [] >>
+  res_tac >> fs []
+QED
+
+val evaluate_nested_seq_append_first = evaluate_nested_seq_cases |> CONJUNCT1
+val evaluate_none_nested_seq_append = evaluate_nested_seq_cases |> CONJUNCT2 |> CONJUNCT1
+val evaluate_not_none_nested_seq_append = evaluate_nested_seq_cases |> CONJUNCT2 |> CONJUNCT2
+
+Definition every_prog_def:
+  (every_prog p (Seq p1 p2) <=>
+    p (Seq p1 p2) /\ every_prog p p1 /\ every_prog p p2) /\
+  (every_prog p (Loop l1 body l2) <=>
+    p (Loop l1 body l2) /\ every_prog p body) /\
+  (every_prog p (If x1 x2 x3 p1 p2 l1) <=>
+    p (If x1 x2 x3 p1 p2 l1) /\ every_prog p p1 /\ every_prog p p2) /\
+  (every_prog p (Mark p1) <=>
+    p (Mark p1) /\ every_prog p p1) /\
+  (every_prog p (Call ret dest args handler) <=>
+    p (Call ret dest args handler) /\
+    (case handler of SOME (n,q,r,l) => every_prog p q ∧ every_prog p r | NONE => T)) /\
+  (every_prog p prog <=> p prog)
+End
+
+Definition comp_syntax_ok_def:
+  comp_syntax_ok p = every_prog
+  (λp. p = Skip ∨
+   ?n m. p = LocValue n m ∨
+   ?n e. p = Assign n e ∨
+   ?n e m. p = LoadByte n e m ∨
+   (?c n m ns v v'. p = If c n (Reg m) (Assign n v) (Assign n v') ns) ∨
+   (?q r. p = Seq q r ∧ comp_syntax_ok q ∧ comp_syntax_ok r)) p
+Termination
+ cheat
+End
+
+
+(*
+Definition comp_syntax_ok_def:
+  comp_syntax_ok p = every_prog
+  (λp. p = Skip ∨
+   ?n m. p = LocValue n m ∨
+   ?n e. p = Assign n e ∨
+   ?n e m. p = LoadByte n e m ∨
+   (?c n ri q r ns. p = If c n ri q r ns ∧ comp_syntax_ok q ∧ comp_syntax_ok r) ∨
+                                          (* could be more restrictive *)
+   (?q r. p = Seq q r ∧ comp_syntax_ok q ∧ comp_syntax_ok r)) p
+Termination
+ cheat
+End
+*)
+
+Theorem comp_syn_ok_basic_cases:
+  comp_syntax_ok Skip /\ (!n m. comp_syntax_ok (LocValue n m)) /\
+  (!n e. comp_syntax_ok (Assign n e)) /\  (!n e m. comp_syntax_ok (LoadByte n e m)) /\
+  (!c n m ns v v'. comp_syntax_ok (If c n (Reg m) (Assign n v) (Assign n v') ns))
+Proof
+  rw [] >>
+  ntac 3 (fs [Once comp_syntax_ok_def, Once every_prog_def])
+QED
+
+
+Theorem comp_syn_ok_seq:
+  !p q. comp_syntax_ok (Seq p q) ==>
+   comp_syntax_ok p /\ comp_syntax_ok q
+Proof
+  rw [] >>
+  fs [Once comp_syntax_ok_def, Once every_prog_def]
+QED
+
+
+Theorem comp_syn_ok_if:
+  comp_syntax_ok (If cmp n m p q ls) ==>
+   ?v v'. p = Assign n v /\ q = Assign n v'
+Proof
+  rw [] >>
+  fs [Once comp_syntax_ok_def, Once every_prog_def]
+QED
+
+
+Theorem comp_syn_ok_seq2:
+  !p q. comp_syntax_ok p /\ comp_syntax_ok q ==>
+   comp_syntax_ok (Seq p q)
+Proof
+  rw [] >>
+  once_rewrite_tac [comp_syntax_ok_def] >>
+  fs [every_prog_def] >>
+  fs [Once comp_syntax_ok_def]
+QED
+
+(*
+Theorem comp_syn_ok_if2:
+  !cmp r1 ri p q ls.
+  comp_syntax_ok p /\  comp_syntax_ok q ==>
+  comp_syntax_ok (If cmp r1 ri p q ls)
+Proof
+  rw [] >>
+  once_rewrite_tac [comp_syntax_ok_def] >>
+  fs [every_prog_def] >>
+  fs [Once comp_syntax_ok_def]
+QED
+*)
+
+Theorem comp_syn_ok_nested_seq:
+  !p q. comp_syntax_ok (nested_seq p) ∧
+   comp_syntax_ok (nested_seq q) ==>
+   comp_syntax_ok (nested_seq (p ++ q))
+Proof
+  Induct >> rw [] >>
+  fs [nested_seq_def] >>
+  drule comp_syn_ok_seq >>
+  strip_tac >> res_tac >> fs [] >>
+  metis_tac [comp_syn_ok_seq2]
+QED
+
+Theorem comp_syn_ok_nested_seq2:
+  !p q. comp_syntax_ok (nested_seq (p ++ q)) ==>
+   comp_syntax_ok (nested_seq p) ∧
+   comp_syntax_ok (nested_seq q)
+Proof
+  Induct >> rw [] >>
+  fs [nested_seq_def, comp_syn_ok_basic_cases] >>
+   drule comp_syn_ok_seq >> strip_tac >> fs [] >>
+   metis_tac [comp_syn_ok_seq2]
+QED
+
+(*
+Definition cut_sets_def:
+  (cut_sets (Seq p q) = inter (cut_sets p) (cut_sets q)) ∧
+  (cut_sets (If _ _ _ p q l) = inter (cut_sets p) (inter (cut_sets q) l)) ∧
+  (cut_sets _ = ARB)
+End
+*)
+
+
+Definition cut_sets_def:
+  (cut_sets l Skip = l) ∧
+  (cut_sets l (LocValue n m) = insert n () l) ∧
+  (cut_sets l (Assign n e) = insert n () l) ∧
+  (cut_sets l (LoadByte n e m) = insert m () l) ∧
+  (cut_sets l (Seq p q) = cut_sets (cut_sets l p) q) ∧
+  (cut_sets l (If _ _ _ p q nl) = cut_sets (cut_sets l p) q) ∧
+  (cut_sets _ _ = ARB)
+End
+
+
+Theorem comp_syn_ok_cut_sets_nested_seq:
+  !p q l. comp_syntax_ok (nested_seq p) ∧
+   comp_syntax_ok (nested_seq q) ==>
+   cut_sets l (nested_seq (p ++ q)) =
+   cut_sets (cut_sets l (nested_seq p)) (nested_seq q)
+Proof
+  Induct >> rw [] >>
+  fs [nested_seq_def]
+  >- fs [cut_sets_def] >>
+  fs [cut_sets_def] >>
+  drule comp_syn_ok_seq >>
+  strip_tac >>
+  res_tac >> fs []
+QED
+
+
+Theorem compile_exp_out_rel_cases:
+  (!ct tmp l (e:'a crepLang$exp) p le ntmp nl.
+    compile_exp ct tmp l e = (p,le,ntmp, nl) ==>
+        comp_syntax_ok (nested_seq p) /\ tmp <= ntmp /\ subspt l nl /\ subspt (cut_sets l (nested_seq p)) nl) /\
+  (!ct tmp l (e:'a crepLang$exp list) p le ntmp nl.
+    compile_exps ct tmp l e = (p,le,ntmp, nl) ==>
+        comp_syntax_ok (nested_seq p) /\ tmp <= ntmp /\ subspt l nl /\ subspt (cut_sets l (nested_seq p)) nl)
+Proof
+  ho_match_mp_tac compile_exp_ind >>
+  rpt conj_tac >> rpt gen_tac >> strip_tac
+  >- (
+   fs [compile_exp_def] >> rveq >>
+   fs [nested_seq_def, comp_syn_ok_basic_cases, cut_sets_def])
+  >- (
+   fs [compile_exp_def] >> rveq >>
+   fs [nested_seq_def, comp_syn_ok_basic_cases, cut_sets_def])
+  >- (
+   fs [compile_exp_def] >> rveq >>
+   conj_tac
+   >- (
+    fs [nested_seq_def] >>
+    match_mp_tac comp_syn_ok_seq2 >>
+    fs [comp_syn_ok_basic_cases]) >>
+   fs [nested_seq_def, cut_sets_def, Once insert_union] >>
+   fs [subspt_union, Once union_num_set_sym])
+  >- (
+   fs [compile_exp_def] >>
+   pairarg_tac >> fs [] >> rveq >>
+   res_tac >> fs [])
+  >- (
+   rpt gen_tac >> strip_tac >>
+   conj_asm1_tac
+   >- (
+    fs [compile_exp_def] >>
+    pairarg_tac >> fs [] >> rveq >> fs [] >>
+    match_mp_tac comp_syn_ok_nested_seq >>
+    fs [] >>
+    fs [nested_seq_def] >>
+    match_mp_tac comp_syn_ok_seq2 >>
+    fs [comp_syn_ok_basic_cases] >>
+    match_mp_tac comp_syn_ok_seq2 >>
+    fs [comp_syn_ok_basic_cases]) >>
+   fs [compile_exp_def] >>
+   pairarg_tac >> fs [] >> rveq >>
+   res_tac >> fs [] >>
+   qmatch_goalsub_rename_tac ‘insert itmp () il’ >>
+   conj_tac
+   >- (
+    qpat_x_assum ‘subspt l il’ assume_tac >>
+    drule subspt_trans >>
+    disch_then (qspec_then ‘insert itmp () il’ mp_tac) >>
+    impl_tac
+    >- (
+     fs [Once insert_union] >> rveq >>
+     fs [subspt_union, Once union_num_set_sym]) >>
+    fs []) >>
+   drule comp_syn_ok_nested_seq2 >>
+   strip_tac >> fs [] >>
+   last_x_assum assume_tac >>
+   drule comp_syn_ok_cut_sets_nested_seq >>
+   disch_then (qspecl_then [‘[Assign itmp le'; LoadByte itmp 0w itmp]’, ‘l’] assume_tac) >>
+   fs [] >> pop_assum kall_tac >>
+   fs [nested_seq_def] >>
+   fs [cut_sets_def] >>
+   fs [Once insert_insert] >>
+   cheat)
+  >- (
+   fs [compile_exp_def] >> rveq >>
+   fs [nested_seq_def, comp_syn_ok_basic_cases, cut_sets_def])
+  >- (
+   fs [Once compile_exp_def] >>
+   pairarg_tac >> fs [] >> rveq >>
+   cases_on ‘e’
+   >- fs [compile_exp_def] >>
+   fs [] >>
+   fs [Once compile_exp_def])
+  >- (
+   rpt gen_tac >> strip_tac >>
+   fs [compile_exp_def] >>
+   pairarg_tac >> fs [] >>
+   pairarg_tac >> fs [] >> rveq >>
+   conj_tac
+   >- (
+    fs [prog_if_def] >>
+    match_mp_tac comp_syn_ok_nested_seq >>
+    conj_tac
+    >- (
+     match_mp_tac comp_syn_ok_nested_seq >>
+     fs []) >>
+    fs [nested_seq_def] >>
+    rpt (match_mp_tac comp_syn_ok_seq2 >>
+         fs [comp_syn_ok_basic_cases])) >>
+   qmatch_goalsub_rename_tac ‘insert ntmp () nl’ >>
+   qmatch_asmsub_rename_tac ‘compile_exp _ _ _ e = (_,_,itmp,il)’ >>
+   qmatch_asmsub_rename_tac ‘compile_exp _ _ _ e' = (_,_,iitmp,_)’ >>
+   cheat (* dxrule subspt_trans >>
+   disch_then (qspec_then ‘insert ntmp () nl’ mp_tac) >>
+   impl_tac
+   >- (
+    drule subspt_trans >>
+    disch_then (qspec_then ‘insert ntmp () nl’ mp_tac) >>
+    impl_tac
+    >- (
+     fs [Once insert_union] >> rveq >>
+     fs [subspt_union, Once union_num_set_sym]) >>
+    fs []) >>
+   fs [] *))
+  >- (
+   fs [compile_exp_def] >>
+   pairarg_tac >> fs []) >>
+  rpt gen_tac >>
+  strip_tac >>
+  cases_on ‘e’ >> fs []
+  >- (
+   fs [compile_exp_def] >>
+   rveq >> fs [] >>
+   fs [nested_seq_def] >>
+   fs [Once comp_syntax_ok_def, every_prog_def, cut_sets_def]) >>
+  pop_assum mp_tac >>
+  once_rewrite_tac [compile_exp_def] >> fs [] >>
+  pairarg_tac >> fs [] >>
+  pairarg_tac >> fs [] >> rveq >>
+  cases_on ‘t’
+  >- (
+   fs [compile_exp_def] >>
+   strip_tac >> rveq >> fs []) >>
+  strip_tac >> fs [] >> rveq >>
+  conj_tac >- metis_tac [subspt_trans, comp_syn_ok_nested_seq] >>
+  conj_tac >-  metis_tac [subspt_trans, comp_syn_ok_nested_seq] >>
+  cheat
+QED
+
+
+val compile_exp_out_rel = compile_exp_out_rel_cases |> CONJUNCT1
+val compile_exps_out_rel = compile_exp_out_rel_cases |> CONJUNCT2
+
+
+Theorem comp_syn_ok_upd_local_clock:
+  !p s res t.
+    evaluate (p,s) = (res,t) /\
+    comp_syntax_ok p ==>
+     t = s with <|locals := t.locals; clock := t.clock|>
+Proof
+  recInduct evaluate_ind >> rw [] >>
+  TRY (fs [Once comp_syntax_ok_def, every_prog_def] >> NO_TAC)
+  >- (
+   fs [evaluate_def] >> rveq >>
+   fs [state_component_equality])
+  >- (
+   fs [evaluate_def] >>
+   FULL_CASE_TAC >> fs [set_var_def] >>
+   rveq >> fs [state_component_equality])
+  >- (
+   fs [evaluate_def] >>
+   every_case_tac >> fs [set_var_def] >> rveq >>
+   fs [state_component_equality])
+  >- (
+   drule comp_syn_ok_seq >>
+   strip_tac >>
+   fs [evaluate_def] >>
+   pairarg_tac >> fs [] >>
+   FULL_CASE_TAC >> fs []  >> rveq >>
+   fs [state_component_equality])
+  >- (
+   drule comp_syn_ok_if >>
+   strip_tac >> rveq >>
+   fs [evaluate_def] >>
+   every_case_tac >> fs [] >> rveq >>
+   fs [state_component_equality] >>
+   fs [evaluate_def, comp_syn_ok_basic_cases] >>
+   every_case_tac >>
+   fs [cut_res_def, cut_state_def, dec_clock_def, set_var_def] >>
+   every_case_tac >> fs [] >> rveq >> fs []) >>
+  fs [evaluate_def] >>
+  FULL_CASE_TAC >> fs [set_var_def] >>
+  rveq >> fs [state_component_equality]
+QED
+
+Definition locals_touched_def:
+  (locals_touched ((Const w):'a loopLang$exp) = []) /\
+  (locals_touched (Var v) = [v]) /\
+  (locals_touched (Lookup name) = []) /\
+  (locals_touched (Load addr) = locals_touched addr) /\
+  (locals_touched (Op op wexps) = FLAT (MAP locals_touched wexps)) /\
+  (locals_touched (Shift sh wexp n) = locals_touched wexp)
+Termination
+  cheat
+End
+
+
+Theorem locals_touched_eq_eval_eq:
+  !s e t.
+   s.globals = t.globals /\ s.memory = t.memory /\ s.mdomain = t.mdomain /\
+   (!n. MEM n (locals_touched e) ==> lookup n s.locals = lookup n t.locals) ==>
+      eval t e = eval s e
+Proof
+  ho_match_mp_tac eval_ind >> rw []
+  >- fs [eval_def]
+  >- fs [eval_def, locals_touched_def]
+  >- fs [eval_def, locals_touched_def]
+  >- (
+   fs [eval_def, locals_touched_def] >>
+   every_case_tac >> fs [mem_load_def])
+  >- (
+   fs [eval_def, locals_touched_def] >>
+   every_case_tac >> fs []
+   >- (
+    ‘the_words (MAP (λa. eval t a) wexps) = SOME x’ suffices_by fs [] >>
+    pop_assum mp_tac >> pop_assum kall_tac >>
+    rpt (pop_assum mp_tac) >>
+    MAP_EVERY qid_spec_tac [‘x’, ‘t’, ‘s’, ‘wexps’] >>
+    Induct >> rw [] >>
+    fs [wordSemTheory.the_words_def,
+        CaseEq "option", CaseEq "word_loc"] >> rveq >> fs [] >>
+    last_x_assum (qspecl_then [‘s’, ‘t’, ‘xs’] mp_tac) >> fs [])
+   >- (
+    ‘the_words (MAP (λa. eval s a) wexps) = SOME x’ suffices_by fs [] >>
+    pop_assum kall_tac >>
+    rpt (pop_assum mp_tac) >>
+    MAP_EVERY qid_spec_tac [‘x’, ‘t’, ‘s’, ‘wexps’] >>
+    Induct >> rw [] >>
+    fs [wordSemTheory.the_words_def,
+        CaseEq "option", CaseEq "word_loc"] >> rveq >> fs [] >>
+    last_x_assum (qspecl_then [‘s’, ‘t’, ‘xs’] mp_tac) >> fs []) >>
+   ‘x = x'’ suffices_by fs [] >>
+   rpt (pop_assum mp_tac) >>
+   MAP_EVERY qid_spec_tac [‘x'’, ‘x’, ‘t’, ‘s’, ‘wexps’] >>
+   Induct >> rw [] >>
+   fs [wordSemTheory.the_words_def,
+       CaseEq "option", CaseEq "word_loc"] >> rveq >> fs [] >>
+   last_x_assum (qspecl_then [‘s’, ‘t’, ‘xs’] mp_tac) >> fs []) >>
+  fs [eval_def, locals_touched_def]
+QED
+
+Definition assigned_vars_def:
+  (assigned_vars Skip = []) ∧
+  (assigned_vars (Assign n e) = [n]) ∧
+  (assigned_vars (LoadByte n w m) = [m]) ∧
+  (assigned_vars (Seq p q) = assigned_vars p ++ assigned_vars q) ∧
+  (assigned_vars (If cmp n r p q ns) = assigned_vars p ++ assigned_vars q) ∧
+  (assigned_vars (LocValue n m) = [n]) ∧
+  (assigned_vars _ = [])
+End
+
+Theorem get_var_imm_add_clk_eq:
+  get_var_imm ri (s with clock := ck) =
+  get_var_imm ri s
+Proof
+  rw [] >>
+  cases_on ‘ri’ >> fs [get_var_imm_def]
+QED
+
+Theorem assigned_vars_nested_seq_split:
+  !p q.
+   comp_syntax_ok (nested_seq p) /\ comp_syntax_ok (nested_seq q) ==>
+    assigned_vars (nested_seq (p ++ q)) =
+    assigned_vars (nested_seq p) ++ assigned_vars (nested_seq q)
+Proof
+  Induct >> rw []
+  >- fs [nested_seq_def, assigned_vars_def] >>
+  fs [nested_seq_def, assigned_vars_def] >>
+  drule comp_syn_ok_seq >> fs []
+QED
+
+Theorem assigned_vars_seq_split:
+  !q p.
+   comp_syntax_ok q /\ comp_syntax_ok p ==>
+    assigned_vars (Seq p q) =
+    assigned_vars p ++ assigned_vars q
+Proof
+  rw [] >> fs [assigned_vars_def]
+QED
+
+
+Theorem comp_exp_assigned_vars_tmp_bound_cases:
+  (!ct tmp l (e :α crepLang$exp) p le ntmp nl n.
+    compile_exp ct tmp l e = (p,le,ntmp,nl) /\
+    MEM n (assigned_vars (nested_seq p)) ==>
+      tmp <= n /\ n < ntmp) /\
+  (!ct tmp l (e :α crepLang$exp list) p le ntmp nl n.
+    compile_exps ct tmp l e = (p,le,ntmp,nl) /\
+    MEM n (assigned_vars (nested_seq p)) ==>
+      tmp <= n /\ n < ntmp)
+Proof
+  ho_match_mp_tac compile_exp_ind >>
+  rpt conj_tac >> rpt gen_tac >> strip_tac
+  >- (
+   fs [compile_exp_def] >> rveq >>
+   fs [nested_seq_def, assigned_vars_def])
+  >- (
+   fs [compile_exp_def] >> rveq >>
+   fs [nested_seq_def, assigned_vars_def])
+  >- (
+   fs [compile_exp_def] >> rveq >>
+   fs [nested_seq_def, assigned_vars_def])
+  >- (
+   fs [compile_exp_def] >> rveq >>
+   pairarg_tac >> fs [])
+  >- (
+   rpt gen_tac >>
+   strip_tac >>
+   fs [compile_exp_def] >> rveq >>
+   pairarg_tac >> fs [] >> rveq >>
+   fs [] >>
+   drule compile_exp_out_rel >>
+   strip_tac >> fs [] >>
+   qmatch_asmsub_abbrev_tac ‘nested_seq (_ ++ q)’ >>
+   ‘comp_syntax_ok (nested_seq q)’ by (
+     fs [Abbr ‘q’, nested_seq_def] >>
+     rpt (match_mp_tac comp_syn_ok_seq2 >>
+          fs [comp_syn_ok_basic_cases])) >>
+   qpat_x_assum ‘comp_syntax_ok (nested_seq p')’ assume_tac >>
+   drule assigned_vars_nested_seq_split >>
+   disch_then (qspec_then ‘q’ mp_tac) >>
+   fs [] >> strip_tac >> fs [] >>
+   pop_assum kall_tac
+   >- (res_tac >> fs []) >>
+   fs [Abbr ‘q’, nested_seq_def] >>
+   fs [assigned_vars_def])
+  >- (
+   fs [compile_exp_def] >> rveq >>
+   fs [nested_seq_def, assigned_vars_def])
+  >- (
+   rpt gen_tac >>
+   strip_tac >>
+   qpat_x_assum ‘compile_exp _ _ _  _ = _’ mp_tac >>
+   once_rewrite_tac [compile_exp_def] >> fs [] >> strip_tac >>
+   pairarg_tac >> fs [])
+  >- (
+   rpt gen_tac >>
+   strip_tac >>
+   fs [compile_exp_def] >>
+   pairarg_tac >> fs [] >>
+   pairarg_tac >> fs [] >> rveq >>
+   fs [prog_if_def] >>
+   ‘tmp <= tmp' /\ tmp' <= tmp''’ by metis_tac [compile_exp_out_rel_cases] >>
+   dxrule compile_exp_out_rel >>
+   dxrule compile_exp_out_rel >>
+   strip_tac >> fs [] >>
+   qmatch_asmsub_abbrev_tac ‘nested_seq (p' ++ p'' ++ q)’ >>
+   ‘comp_syntax_ok (nested_seq q)’ by (
+     fs [Abbr ‘q’, nested_seq_def] >>
+     rpt (match_mp_tac comp_syn_ok_seq2 >>
+          fs [comp_syn_ok_basic_cases])) >>
+   strip_tac >>
+   qpat_x_assum ‘comp_syntax_ok (nested_seq p')’ assume_tac >>
+   drule assigned_vars_nested_seq_split >>
+   disch_then (qspec_then ‘p'' ++ q’ mp_tac) >>
+   fs [] >>
+   pop_assum mp_tac >>
+   drule comp_syn_ok_nested_seq >>
+   disch_then (qspec_then ‘q’ mp_tac) >>
+   fs [] >>
+   ntac 3 strip_tac >>
+   fs []
+   >- (res_tac >> fs []) >>
+   ntac 3 (pop_assum kall_tac) >>
+   drule assigned_vars_nested_seq_split >>
+   disch_then (qspec_then ‘q’ mp_tac) >>
+   fs [] >>
+   strip_tac >> fs []
+   >- (res_tac >> fs []) >>
+   pop_assum kall_tac >>
+   fs [Abbr ‘q’, nested_seq_def] >>
+   pop_assum kall_tac >>
+   drule comp_syn_ok_seq >>
+   strip_tac >>
+   drule assigned_vars_seq_split >>
+   disch_then (qspec_then ‘Assign (tmp'' + 1) le'’ mp_tac) >>
+   fs [] >> strip_tac >> fs [] >>
+   pop_assum kall_tac
+   >- fs [assigned_vars_def] >>
+   drule comp_syn_ok_seq >>
+   strip_tac >>
+   drule assigned_vars_seq_split >>
+   disch_then (qspec_then ‘Assign (tmp'' + 2) le''’ mp_tac) >>
+   fs [] >> strip_tac >> fs [] >>
+   pop_assum kall_tac
+   >- fs [assigned_vars_def] >>
+   drule comp_syn_ok_seq >>
+   strip_tac >>
+   drule assigned_vars_seq_split >>
+   disch_then (qspec_then ‘If cmp (tmp'' + 1) (Reg (tmp'' + 2))
+             (Assign (tmp'' + 1) (Const 1w)) (Assign (tmp'' + 1) (Const 0w))
+             (insert (tmp'' + 1) () l'')’ mp_tac) >>
+   fs [] >> strip_tac >> fs [] >>
+   pop_assum kall_tac >>
+   fs [assigned_vars_def])
+  >- (
+   fs [compile_exp_def] >> rveq >>
+   pairarg_tac >> fs []) >>
+  rpt gen_tac >>
+  strip_tac >>
+  pop_assum mp_tac >> fs [] >>
+  once_rewrite_tac [compile_exp_def] >>
+  cases_on ‘e’ >> fs []
+  >- (
+   fs [compile_exp_def] >> rveq >>
+   fs [nested_seq_def, assigned_vars_def]) >>
+  pop_assum mp_tac >>
+  once_rewrite_tac [compile_exp_def] >>
+  fs [] >>
+  pairarg_tac >> fs [] >>
+  pairarg_tac >> fs [] >>
+  strip_tac >> rveq >> fs [] >>
+  strip_tac >>
+  ‘tmp <= tmp' /\ tmp' <= ntmp’ by metis_tac [compile_exp_out_rel_cases] >>
+  dxrule compile_exp_out_rel >>
+  dxrule compile_exps_out_rel >>
+  rpt strip_tac >> fs [] >>
+  drule assigned_vars_nested_seq_split >>
+  disch_then (qspec_then ‘p1’ mp_tac) >>
+  fs [] >>
+  strip_tac >> fs [] >>
+  res_tac >> fs []
+QED
+
+val comp_exp_assigned_vars_tmp_bound = comp_exp_assigned_vars_tmp_bound_cases |> CONJUNCT1
+val comp_exps_assigned_vars_tmp_bound = comp_exp_assigned_vars_tmp_bound_cases |> CONJUNCT2
+
+Definition var_cexp_def:
+  (var_cexp (Const w:'a crepLang$exp) = ([]:num list)) ∧
+  (var_cexp (Var v) = [v]) ∧
+  (var_cexp (Label f) = []) ∧
+  (var_cexp (Load e) = var_cexp e) ∧
+  (var_cexp (LoadByte e) = var_cexp e) ∧
+  (var_cexp (LoadGlob a) = []) ∧
+  (var_cexp (Op bop es) = FLAT (MAP var_cexp es)) ∧
+  (var_cexp (Cmp c e1 e2) = var_cexp e1 ++ var_cexp e2) ∧
+  (var_cexp (Shift sh e num) = var_cexp e)
+Termination
+  wf_rel_tac `measure (\e. crepLang$exp_size ARB e)` >>
+  rpt strip_tac >>
+  imp_res_tac crepLangTheory.MEM_IMP_exp_size >>
+  TRY (first_x_assum (assume_tac o Q.SPEC `ARB`)) >>
+  decide_tac
+End
+
+
+Theorem compile_exp_le_tmp_domain_cases:
+  (!ct tmp l (e:'a crepLang$exp) p le tmp' l' n.
+    ctxt_max ct.vmax ct.vars /\
+    compile_exp ct tmp l e = (p,le,tmp', l') /\ ct.vmax < tmp /\
+    (!n. MEM n (var_cexp e) ==> ?m. FLOOKUP ct.vars n = SOME m /\ m ∈ domain l) /\
+    MEM n (locals_touched le) ==> n < tmp' /\ n ∈ domain l') /\
+  (!ct tmp l (es:'a crepLang$exp list) p les tmp' l' n.
+    ctxt_max ct.vmax ct.vars /\
+    compile_exps ct tmp l es = (p,les,tmp', l') /\ ct.vmax < tmp /\
+    (!n. MEM n (FLAT (MAP var_cexp es)) ==> ?m. FLOOKUP ct.vars n = SOME m /\ m ∈ domain l) /\
+    MEM n (FLAT (MAP locals_touched les)) ==> n < tmp' /\ n ∈ domain l')
+Proof
+  ho_match_mp_tac compile_exp_ind >>
+  rpt conj_tac >> rpt gen_tac >> strip_tac
+  >- (
+   fs [compile_exp_def] >> rveq >>
+   fs [locals_touched_def])
+  >- (
+   fs [compile_exp_def] >> rveq >>
+   fs [locals_touched_def, find_var_def, var_cexp_def, ctxt_max_def] >>
+   rfs [] >> rveq >> res_tac >> fs [])
+  >- (
+   fs [compile_exp_def] >> rveq >>
+   fs [locals_touched_def, var_cexp_def])
+  >- (
+   fs [compile_exp_def] >>
+   pairarg_tac >> fs [] >> rveq >>
+   fs [var_cexp_def, locals_touched_def])
+  >- (
+   fs [compile_exp_def] >>
+   pairarg_tac >> fs [] >> rveq >>
+   fs [var_cexp_def, locals_touched_def])
+  >- (
+   fs [compile_exp_def] >> rveq >>
+   fs [var_cexp_def, locals_touched_def])
+  >- (
+   rpt gen_tac >>
+   strip_tac >>
+   qpat_x_assum ‘compile_exp _ _ _ _ = _’ mp_tac >>
+   once_rewrite_tac [compile_exp_def] >>
+   strip_tac >> fs [] >>
+   pairarg_tac >> fs [] >> rveq >>
+   fs [locals_touched_def, var_cexp_def, ETA_AX])
+  >- (
+   rpt gen_tac >>
+   strip_tac >>
+   fs [compile_exp_def] >>
+   pairarg_tac >> fs [] >> rveq >>
+   pairarg_tac >> fs [] >> rveq >>
+   fs [var_cexp_def, locals_touched_def])
+  >- (
+   rpt gen_tac >>
+   strip_tac >>
+   fs [compile_exp_def] >>
+   pairarg_tac >> fs [] >> rveq >>
+   fs [locals_touched_def, var_cexp_def]) >>
+  rpt gen_tac >>
+  strip_tac >>
+  qpat_x_assum ‘compile_exps _ _ _ _ = _’ mp_tac >>
+  once_rewrite_tac [compile_exp_def] >>
+  cases_on ‘es’ >> fs [] >> rveq
+  >- (
+   strip_tac >> rveq >>
+   fs [MAP]) >>
+  strip_tac >>
+  pairarg_tac >> fs [] >>
+  pairarg_tac >> fs [] >> rveq >>
+  ‘tmp <= tmp'' /\ tmp'' <= tmp' /\ subspt l l'' /\ subspt l'' l'’ by
+    metis_tac [compile_exp_out_rel_cases] >>
+  fs [MAP]
+  >- (
+   res_tac >> fs [subspt_domain] >>
+   metis_tac [SUBSET_IMP]) >>
+  last_x_assum match_mp_tac >>
+  fs [] >>
+  rw [] >>
+  res_tac >> fs [subspt_domain] >>
+  metis_tac [SUBSET_IMP]
+QED
+
+val compile_exp_le_tmp_domain = compile_exp_le_tmp_domain_cases |> CONJUNCT1
+val compile_exps_le_tmp_domain_cases = compile_exp_le_tmp_domain_cases |> CONJUNCT2
+
+Theorem foo:
+  n ∈ domain l /\  comp_syntax_ok p ==>
+  n ∈ domain (cut_sets l p)
+Proof
+  cheat
+QED
+
+Theorem foo2:
+  comp_syntax_ok p ==>
+  subspt  l (cut_sets l p)
+Proof
+  cheat
+QED
+
+Theorem abc:
+  !(p:'a prog) (q:'a prog) l. comp_syntax_ok p /\ comp_syntax_ok q /\
+  subspt l (cut_sets (cut_sets l p) q) ==> subspt l (cut_sets l p)
+Proof
+  Induct >> rw [] >>
+  TRY (fs [Once comp_syntax_ok_def, every_prog_def] >> NO_TAC)
+  >- fs [cut_sets_def]
+  >- (
+   fs [cut_sets_def] >>
+   fs [Once insert_union] >>
+   fs [subspt_union, Once union_num_set_sym]) >>
+   cheat
+QED
+
+Theorem comp_syn_ok_lookup_locals_eq:
+  !p s res t l n.
+   evaluate (p,s) = (res,t) /\
+   comp_syntax_ok p /\ n ∈ domain l /\
+   subspt l (cut_sets l p) /\
+    ~MEM n (assigned_vars p) ==>
+  lookup n t.locals = lookup n s.locals
+Proof
+  recInduct evaluate_ind >> rw [] >>
+  TRY (fs [Once comp_syntax_ok_def, every_prog_def] >> NO_TAC)
+  >- fs [evaluate_def]
+  >- (
+   fs [evaluate_def] >>
+   every_case_tac >> fs [] >> rveq >>
+   fs [set_var_def, assigned_vars_def, lookup_insert])
+  >- (
+   fs [evaluate_def] >>
+   every_case_tac >> fs [] >> rveq >>
+   fs [set_var_def, assigned_vars_def, lookup_insert])
+  >- (
+   drule comp_syn_ok_seq >>
+   strip_tac >>
+   fs [evaluate_def, assigned_vars_def] >>
+   pairarg_tac >> fs [AllCaseEqs ()] >> rveq >> fs []
+   >- (
+    fs [cut_sets_def] >>
+    qpat_x_assum ‘comp_syntax_ok c1’ assume_tac >>
+    drule abc >>
+    disch_then (qspecl_then [‘c2’, ‘l’] mp_tac) >>
+    fs [] >>
+    strip_tac >>
+    first_x_assum drule >>
+    fs [] >> strip_tac >>
+    drule foo >>
+    disch_then (qspec_then ‘c1’ mp_tac) >>
+    fs [] >> strip_tac >>
+    last_x_assum drule >> fs [] >>
+    metis_tac [foo2]) >>
+   first_x_assum drule >>
+   fs [] >> metis_tac [foo2])
+  >- (
+   drule comp_syn_ok_if >>
+   strip_tac >>
+   fs [evaluate_def, assigned_vars_def] >>
+   fs [AllCaseEqs()]  >> rveq >> fs [cut_sets_def, domain_inter] >>
+   cases_on ‘word_cmp cmp x y’ >> fs []
+   >- (
+    cases_on ‘evaluate (c1,s)’ >> fs [] >>
+    fs [cut_res_def, cut_state_def, AllCaseEqs()] >>
+    fs [evaluate_def] >>
+    FULL_CASE_TAC >> fs [cut_res_def] >>
+    fs [set_var_def, dec_clock_def] >>
+    FULL_CASE_TAC >> fs [] >> rveq >>
+    fs [comp_syn_ok_basic_cases, cut_sets_def, assigned_vars_def] >>
+    rfs [Once insert_insert] >>
+    res_tac >> fs [] >> cheat) >>
+   cases_on ‘evaluate (c2,s)’ >> fs [] >>
+   fs [cut_res_def, cut_state_def, AllCaseEqs()] >>
+   fs [evaluate_def] >>
+   FULL_CASE_TAC >> fs [cut_res_def] >>
+   fs [set_var_def, dec_clock_def] >>
+   FULL_CASE_TAC >> fs [] >> rveq >>
+   fs [comp_syn_ok_basic_cases, cut_sets_def, assigned_vars_def] >>
+   rfs [Once insert_insert] >>
+   res_tac >> fs [] >> cheat) >>
+  fs [dec_clock_def, lookup_inter] >>
+  fs [evaluate_def] >>
+  every_case_tac >> fs [] >> rveq >>
+  fs [set_var_def, assigned_vars_def, lookup_insert]
+QED
+
+
+
+Theorem nested_seq_pure_evaluation:
+  !p q t r st l m e v.
+  evaluate (nested_seq (p ++ q),t) = (NONE,r) /\
+  evaluate (nested_seq p,t) = (NONE,st) /\
+  comp_syntax_ok (nested_seq p) /\
+  comp_syntax_ok (nested_seq q) /\
+  subspt l (cut_sets l (nested_seq p)) /\
+  subspt (cut_sets l (nested_seq p)) (cut_sets (cut_sets l (nested_seq p)) (nested_seq q)) /\
+  (!n. MEM n (assigned_vars (nested_seq p)) ==> n < m) /\
+  (!n. MEM n (assigned_vars (nested_seq q)) ==> m <= n) /\
+  (!n. MEM n (locals_touched e) ==> n < m /\ n ∈ domain l) /\
+   eval st e = SOME v ==>
+    eval r e = SOME v
+Proof
+  rw [] >>
+  drule_all evaluate_nested_seq_append_first >> strip_tac >>
+  drule comp_syn_ok_upd_local_clock >>
+  fs [] >> strip_tac >>
+  ‘st.globals = r.globals /\ st.memory = r.memory /\
+   st.mdomain = r.mdomain’ by fs [state_component_equality] >>
+  drule locals_touched_eq_eval_eq >> fs [] >>
+  disch_then (qspec_then ‘e’ mp_tac) >> fs [] >>
+  impl_tac
+  >- (
+   rw []  >>
+   drule comp_syn_ok_lookup_locals_eq >>
+   fs [] >>
+   disch_then (qspecl_then [‘l’, ‘n’] mp_tac) >>
+   impl_tac
+   >- (
+    fs [foo2] >> CCONTR_TAC >> fs [] >>
+    res_tac >> fs []) >>
+   fs []) >> fs []
+QED
+
+
+Theorem comp_exp_preserves_eval:
+  ∀s e v (t :('a, 'b) state) ctxt tmp l.
+  eval s e = SOME v /\
+  state_rel s t /\ mem_rel ctxt s.memory t.memory /\
+  globals_rel ctxt s.globals t.globals /\
+  code_rel ctxt s.code t.code /\
+  locals_rel ctxt l s.locals t.locals /\
+  ctxt.vmax < tmp ==>
+    let (p,le, tmp, l) = compile_exp ctxt tmp l e in
+     ?st. evaluate (nested_seq p,t) = (NONE,st) /\
+     eval st le = SOME (wlab_wloc ctxt v) /\
+     state_rel s st /\ mem_rel ctxt s.memory st.memory /\
+     globals_rel ctxt s.globals st.globals /\
+     code_rel ctxt s.code st.code /\
+     locals_rel ctxt l s.locals st.locals
+Proof
+  ho_match_mp_tac crepSemTheory.eval_ind >>
+  rpt conj_tac >> rpt gen_tac >> strip_tac
+  >- (
+   rename [‘Const w’] >>
+   fs [crepSemTheory.eval_def] >> rveq >>
+   fs [compile_exp_def] >>
+   fs [nested_seq_def, evaluate_def, eval_def, wlab_wloc_def])
+  >- (
+   rename [‘eval s (Var vname)’] >>
+   fs [crepSemTheory.eval_def] >> rveq >>
+   pairarg_tac >> fs [] >>
+   fs [compile_exp_def] >> rveq >>
+   fs [nested_seq_def, evaluate_def, find_var_def] >>
+   imp_res_tac locals_rel_intro >>
+   fs [eval_def])
+  >- (
+   rename [‘eval s (Label fname)’] >>
+   fs [crepSemTheory.eval_def, CaseEq "option"] >> rveq >>
+   pairarg_tac >> fs [compile_exp_def] >> rveq >>
+   fs [nested_seq_def, evaluate_def, find_lab_def] >>
+   cases_on ‘v1’ >> rveq >>
+   imp_res_tac code_rel_intro >>
+   fs [eval_def, set_var_def, domain_lookup, wlab_wloc_def,
+       state_rel_def] >>
+   fs [locals_rel_def, SUBSET_INSERT_RIGHT] >> rw [] >>
+   first_x_assum drule >> fs [] >>
+   strip_tac >> fs [] >>
+   fs [lookup_insert] >>
+   TOP_CASE_TAC >> fs [] >>
+   fs [ctxt_max_def] >>
+   first_x_assum drule >> fs [])
+  >- (
+   rename [‘eval s (Load e)’] >>
+   fs [crepSemTheory.eval_def] >>
+   TOP_CASE_TAC >> fs [] >>
+   TOP_CASE_TAC >> fs [] >>
+   rw [] >>
+   pairarg_tac >> fs [] >>
+   fs [compile_exp_def] >>
+   pairarg_tac >> fs [] >> rveq >>
+   last_x_assum drule_all >>
+   pairarg_tac >> fs [] >> rveq >>
+   strip_tac >> fs [] >>
+   fs [loopSemTheory.eval_def, wlab_wloc_def] >>
+   fs [crepSemTheory.mem_load_def, loopSemTheory.mem_load_def] >> rveq >>
+   imp_res_tac state_rel_intro >>
+   imp_res_tac mem_rel_intro >>
+   last_x_assum (qspec_then ‘c’ mp_tac) >> fs [])
+  >- (
+   rename [‘eval s (LoadByte e)’] >>
+   fs [crepSemTheory.eval_def] >>
+   TOP_CASE_TAC >> fs [] >>
+   TOP_CASE_TAC >> fs [] >>
+   TOP_CASE_TAC >> fs [] >>
+   rw [] >>
+   pairarg_tac >> fs [] >>
+   fs [compile_exp_def] >>
+   pairarg_tac >> fs [] >> rveq >>
+   last_x_assum drule_all >>
+   pairarg_tac >> fs [] >> rveq >>
+   strip_tac >> fs [] >>
+   drule evaluate_none_nested_seq_append >>
+   disch_then (qspec_then
+               ‘[Assign tmp' le; LoadByte tmp' 0w tmp']’ mp_tac) >>
+   strip_tac >> fs [] >>
+   fs [nested_seq_def, loopSemTheory.evaluate_def] >>
+   fs [set_var_def, wlab_wloc_def] >>
+   fs [panSemTheory.mem_load_byte_def, CaseEq "word_lab",
+       wordSemTheory.mem_load_byte_aux_def] >>
+   imp_res_tac mem_rel_intro >>
+   last_x_assum (qspec_then ‘byte_align c’ (mp_tac o GSYM)) >>
+   strip_tac >> fs [] >>
+   last_x_assum (qspec_then ‘byte_align c’ (mp_tac o GSYM)) >>
+   strip_tac >> fs [wlab_wloc_def] >>
+   imp_res_tac state_rel_intro >>
+   fs [eval_def, state_rel_def] >>
+   imp_res_tac compile_exp_out_rel >>
+   fs [locals_rel_def, SUBSET_INSERT_RIGHT] >> rw [] >>
+   first_x_assum drule >> fs [] >>
+   strip_tac >> fs [] >>
+   fs [lookup_insert] >>
+   TOP_CASE_TAC >> fs [] >>
+   fs [ctxt_max_def] >>
+   first_x_assum drule >> fs [])
+  >- (
+   rename [‘eval s (LoadGlob gadr)’] >>
+   fs [crepSemTheory.eval_def] >>
+   pairarg_tac >> fs [] >>
+   fs [compile_exp_def] >> rveq >>
+   fs [nested_seq_def, loopSemTheory.evaluate_def] >>
+   fs [eval_def] >>
+   imp_res_tac globals_rel_intro >>
+   fs [])
+  >- (
+   rename [‘eval s (Op op es)’] >>
+   rw [] >>
+   pairarg_tac >> fs [] >>
+   fs [Once compile_exp_def] >> fs [] >>
+   pairarg_tac >> fs [] >> rveq >>
+   fs [crepSemTheory.eval_def, CaseEq "option"] >> rveq >>
+   fs [loopSemTheory.eval_def] >>
+   cases_on ‘evaluate (nested_seq p,t)’ >> fs [] >>
+   ‘q = NONE /\ the_words (MAP (λa. eval r a) les) =
+    SOME ((MAP (λw. case w of Word n =>  n | Label v1 => ARB) ws))’ by (
+     qpat_x_assum ‘word_op _ _ = _’ kall_tac >>
+     rpt (pop_assum mp_tac) >>
+     MAP_EVERY qid_spec_tac [‘t’, ‘p’, ‘les’ , ‘tmp’, ‘l’,‘ws’, ‘es’] >>
+     Induct
+     >- (
+      rw [] >>
+      fs [OPT_MMAP_def] >> rveq >>
+      fs [compile_exp_def] >> rveq >>
+      fs [nested_seq_def, loopSemTheory.evaluate_def, wordSemTheory.the_words_def]) >>
+     rpt gen_tac >>
+     once_rewrite_tac [compile_exp_def] >>
+     ntac 11 strip_tac >> fs [] >>
+     fs [OPT_MMAP_def] >> rveq >>
+     pairarg_tac >> fs [] >>
+     pairarg_tac >> fs [] >> rveq >>
+     first_x_assum (qspec_then ‘h’ mp_tac) >>
+     fs [] >>
+     disch_then drule_all >>
+     strip_tac >> pairarg_tac >> fs [] >> rveq >>
+     qmatch_asmsub_rename_tac ‘compile_exp _ _ _ h = (p,le,itmp,il)’ >>
+     qmatch_asmsub_rename_tac ‘compile_exps _ _ _ _ = (fp,les,ntmp,nl)’ >>
+     last_x_assum (qspecl_then
+                   [‘il’, ‘itmp’, ‘les’, ‘fp’, ‘st’] mp_tac) >>
+     fs [] >>
+     imp_res_tac compile_exp_out_rel >>
+     fs [] >>
+     impl_tac
+     >- (
+      imp_res_tac evaluate_none_nested_seq_append >>
+      fs []) >>
+     strip_tac >> fs [] >>
+     cases_on ‘h'’ >> fs [] >>
+     fs [wordSemTheory.the_words_def] >>
+     ‘eval r le = eval st le’ suffices_by fs [wlab_wloc_def] >>
+     drule evaluate_nested_seq_append_first >>
+     disch_then drule >>
+     strip_tac >> fs [] >>
+     imp_res_tac compile_exps_out_rel >>
+     drule comp_syn_ok_upd_local_clock >>
+     fs [] >> strip_tac >>
+     drule nested_seq_pure_evaluation >>
+     disch_then drule >> fs [wlab_wloc_def] >>
+     disch_then (qspecl_then [‘il’, ‘itmp’, ‘le’, ‘Word c’] mp_tac) >>
+     impl_tac
+     >- (
+      fs [foo2] >>
+      drule comp_exp_assigned_vars_tmp_bound >> fs [] >>
+      strip_tac >>
+      drule comp_exps_assigned_vars_tmp_bound >> fs [] >>
+      strip_tac >>
+      gen_tac >>
+      strip_tac >> fs [] >>
+      imp_res_tac locals_rel_intro >>
+      drule compile_exp_le_tmp_domain >>
+      disch_then (qspecl_then [‘tmp’, ‘l’, ‘h’, ‘p’, ‘le’,
+                               ‘itmp’, ‘il’, ‘n’] mp_tac) >>
+      fs [] >>
+      impl_tac
+      >- (rw [] >> cheat) >>
+      fs []) >>
+     fs []) >>
+   fs [wlab_wloc_def] >>
+   pop_assum kall_tac >>
+   pop_assum kall_tac >>
+   ntac 8 (pop_assum mp_tac) >>
+   pop_assum kall_tac >>
+   pop_assum kall_tac >>
+   pop_assum mp_tac >>
+   pop_assum mp_tac >>
+   MAP_EVERY qid_spec_tac [‘t’, ‘p’, ‘les’ , ‘tmp’, ‘l’, ‘ws’, ‘es’] >>
+   Induct
+   >- (
+    rw [] >>
+    fs [OPT_MMAP_def] >> rveq >>
+    fs [compile_exp_def] >> rveq >>
+    fs [nested_seq_def, loopSemTheory.evaluate_def, wordSemTheory.the_words_def]) >>
+   rpt gen_tac >>
+   once_rewrite_tac [compile_exp_def] >>
+   ntac 10 strip_tac >> fs [] >>
+   last_x_assum mp_tac >>
+   pairarg_tac >> fs [] >>
+   pairarg_tac >> fs [] >> rveq >>
+   last_x_assum (qspec_then ‘h’ mp_tac) >>
+   fs [] >>
+   fs [OPT_MMAP_def] >> rveq >>
+   disch_then drule_all >>
+   pairarg_tac >> fs [] >> rveq >>
+   strip_tac >> fs [] >>
+   disch_then drule >>
+   disch_then (qspecl_then [‘l''’, ‘tmp''’, ‘les'’, ‘p1’] mp_tac) >>
+   fs [] >>
+   imp_res_tac compile_exp_out_rel >>
+   fs [] >>
+   imp_res_tac evaluate_nested_seq_append_first >>
+   fs [])
+  >- (
+   rw [] >>
+   fs [crepSemTheory.eval_def, CaseEq "option", CaseEq "word_lab"] >>
+   rveq >> fs [] >>
+   pairarg_tac >> fs [] >>
+   fs [compile_exp_def] >>
+   pairarg_tac >> fs [] >>
+   pairarg_tac >> fs [] >>
+   rveq >> fs [] >>
+   fs [prog_if_def] >>
+   last_x_assum drule_all >>
+   pairarg_tac >> fs [] >>
+   strip_tac >> fs [] >> rveq >>
+   qmatch_asmsub_rename_tac ‘compile_exp _ _ _ e = (p1,le1,tmp1,l1)’ >>
+   qmatch_asmsub_rename_tac ‘compile_exp _ _ _ e' = (p2,le2,tmp2,l2)’ >>
+   last_x_assum (qspecl_then [‘st’, ‘ctxt’, ‘tmp1’, ‘l1’] mp_tac) >>
+   fs [] >>
+   imp_res_tac compile_exp_out_rel >> fs [] >>
+   strip_tac >> fs [] >>
+   qmatch_goalsub_abbrev_tac ‘nested_seq (_ ++ _ ++ np)’ >>
+   qpat_x_assum ‘evaluate (_,st) = _’ mp_tac >>
+   drule evaluate_none_nested_seq_append >>
+   disch_then (qspec_then ‘p2 ++ np’ mp_tac) >>
+   strip_tac >> fs [] >>
+   pop_assum kall_tac >>
+   strip_tac >>
+   drule evaluate_none_nested_seq_append >>
+   disch_then (qspec_then ‘np’ mp_tac) >>
+   strip_tac >> fs [] >>
+   pop_assum kall_tac >>
+   fs [Abbr ‘np’, nested_seq_def] >>
+   fs [evaluate_def] >>
+   pairarg_tac >> fs [] >>
+   pairarg_tac >> fs [] >>
+   pairarg_tac >> fs [] >>
+   rfs [] >>
+   ‘eval st' le1 = eval st le1’ by (
+     ‘evaluate (nested_seq (p1 ++ p2),t) = (NONE,st')’ by
+       metis_tac [evaluate_none_nested_seq_append] >>
+     drule nested_seq_pure_evaluation >>
+     fs [] >> fs [wlab_wloc_def] >>
+     disch_then (qspecl_then [‘l1’, ‘tmp1’, ‘le1’, ‘Word w1’] mp_tac) >>
+     impl_tac
+     >- (
+      fs [foo2] >>
+      imp_res_tac comp_exp_assigned_vars_tmp_bound >> fs [] >>
+      gen_tac >>
+      strip_tac >> fs [] >>
+      imp_res_tac locals_rel_intro >>
+      drule compile_exp_le_tmp_domain >>
+      disch_then (qspecl_then [‘tmp’, ‘l’, ‘e’, ‘p1’, ‘le1’,
+                               ‘tmp1’, ‘l1’, ‘n’] mp_tac) >>
+      fs [] >>
+      impl_tac
+      >- (rw [] >> cheat) >>
+      fs []) >> fs []) >>
+     fs [] >> rfs [] >> rveq >>
+     fs [wlab_wloc_def, loopSemTheory.set_var_def,
+         loopSemTheory.eval_def] >>
+     ‘eval (st' with locals := insert (tmp2 + 1) (Word w1) st'.locals)
+      le2 = eval st' le2’ by (
+       ho_match_mp_tac locals_touched_eq_eval_eq >>
+       fs [] >> rw [] >> fs [lookup_insert] >>
+       TOP_CASE_TAC >> fs [] >>
+       imp_res_tac locals_rel_intro >>
+       drule compile_exp_le_tmp_domain >>
+       disch_then (qspecl_then [‘tmp1’, ‘l1’, ‘e'’, ‘p2’, ‘le2’,
+                                ‘tmp2’, ‘l2’, ‘n’] mp_tac) >>
+       impl_tac
+       >- (
+        conj_tac >- fs [] >>
+        conj_tac >- fs [] >>
+        conj_tac >- cheat >>
+        fs []) >>
+       fs []) >>
+     fs [] >> rfs [] >> rveq >>
+     fs [lookup_insert] >>
+     fs [get_var_imm_def] >>
+     cases_on ‘word_cmp cmp w1 w2’ >>
+     fs [loopSemTheory.evaluate_def, loopSemTheory.eval_def,
+         loopSemTheory.set_var_def] >> (
+     fs [cut_res_def] >>
+     fs [cut_state_def] >>
+     imp_res_tac locals_rel_intro >>
+     fs [SUBSET_INSERT_RIGHT] >>
+     cases_on ‘st'.clock = 0’ >- cheat >>
+     fs [dec_clock_def] >> rveq >> fs [] >>
+     fs [lookup_inter] >>
+     conj_tac >- EVAL_TAC >>
+     conj_tac >- cheat (* clock is changed *) >>
+     fs [locals_rel_def, domain_inter, SUBSET_INSERT_RIGHT] >>
+     rw [] >>
+     fs [lookup_inter, lookup_insert] >>
+     res_tac >> fs [] >> rveq >> fs [] >>
+     ‘n <= tmp2’ by (fs [ctxt_max_def] >> res_tac >> fs []) >>
+     fs [domain_lookup])) >>
+  rw [] >>
+  fs [crepSemTheory.eval_def, CaseEq "option", CaseEq "word_lab"] >>
+  rveq >> fs [] >>
+  pairarg_tac >> fs [compile_exp_def] >>
+  pairarg_tac >> fs [] >> rveq >>
+  fs [loopSemTheory.evaluate_def] >>
+  last_x_assum drule_all >>
+  strip_tac >> rfs [] >>
+  fs [loopSemTheory.eval_def, wlab_wloc_def]
+QED
+
+(*
+(* with clock *)
+
+Theorem comp_syn_ok_lookup_locals_eq:
+  !p s res t n.
+   evaluate (p,s) = (res,t) /\ t.clock <> 0 /\
+   comp_syntax_ok p /\ n ∈ domain (cut_sets p) /\
+    ~MEM n (assigned_vars p) ==>
+  lookup n t.locals = lookup n s.locals
+Proof
+  recInduct evaluate_ind >> rw [] >>
+  TRY (fs [Once comp_syntax_ok_def, every_prog_def] >> NO_TAC)
+  >- fs [evaluate_def]
+  >- (
+   fs [evaluate_def] >>
+   every_case_tac >> fs [] >> rveq >>
+   fs [set_var_def, assigned_vars_def, lookup_insert])
+  >- (
+   fs [evaluate_def] >>
+   every_case_tac >> fs [] >> rveq >>
+   fs [set_var_def, assigned_vars_def, lookup_insert])
+  >- (
+   drule comp_syn_ok_seq >>
+   fs [cut_sets_def, domain_inter] >>
+   fs [evaluate_def, assigned_vars_def] >>
+   pairarg_tac >> fs [AllCaseEqs ()] >> rveq >> fs [] >>
+   dxrule evaluate_clock >> dxrule evaluate_clock >>
+   fs [])
+  >- (
+   drule comp_syn_ok_if >>
+   strip_tac >>
+   fs [evaluate_def, assigned_vars_def] >>
+   fs [AllCaseEqs()]  >> rveq >> fs [cut_sets_def, domain_inter] >>
+   cases_on ‘word_cmp cmp x y’ >> fs []
+   >- (
+    cases_on ‘evaluate (c1,s)’ >> fs [] >>
+    fs [get_var_imm_add_clk_eq,
+        cut_res_def, cut_state_def, AllCaseEqs()] >>
+    rveq >> res_tac >> fs [] >>
+    fs [dec_clock_def, lookup_inter] >>
+    fs [domain_lookup] >> TOP_CASE_TAC >> fs []) >>
+   cases_on ‘evaluate (c2,s)’ >> fs [] >>
+   fs [cut_res_def, cut_state_def, AllCaseEqs()] >>
+   rveq >> fs [dec_clock_def, lookup_inter] >>
+   fs [domain_lookup] >> TOP_CASE_TAC >> fs []) >>
+  fs [evaluate_def] >>
+  every_case_tac >> fs [] >> rveq >>
+  fs [set_var_def, assigned_vars_def, lookup_insert]
+QED
+
+Theorem state_rel_add_clock:
+  state_rel s t ==>
+  ∃ck. state_rel s (t with clock := ck + t.clock)
+Proof
+  rw [] >>
+  qexists_tac ‘0’ >>
+  fs [state_component_equality, state_rel_def]
+QED
+
+
+Theorem comp_exp_preserves_eval:
+  ∀s e v (t :('a, 'b) state) ctxt tmp l.
+  eval s e = SOME v /\
+  state_rel s t /\ mem_rel ctxt s.memory t.memory /\
+  globals_rel ctxt s.globals t.globals /\
+  code_rel ctxt s.code t.code /\
+  locals_rel ctxt s.locals t.locals /\
+  ctxt.vmax < tmp ==>
+    let (p,le, tmp, l) = compile_exp ctxt tmp l e in
+     ?ck st. evaluate (nested_seq p,t with clock := t.clock + ck) = (NONE,st) /\
+     eval st le = SOME (wlab_wloc ctxt v) /\
+     state_rel s st /\ mem_rel ctxt s.memory st.memory /\
+     globals_rel ctxt s.globals st.globals /\
+     code_rel ctxt s.code st.code /\
+     locals_rel ctxt s.locals st.locals
+Proof
+  ho_match_mp_tac crepSemTheory.eval_ind >>
+  rpt conj_tac >> rpt gen_tac >> strip_tac
+  >- (
+   rename [‘Const w’] >>
+   fs [crepSemTheory.eval_def] >> rveq >>
+   fs [compile_exp_def] >>
+   fs [nested_seq_def, evaluate_def, eval_def,
+       wlab_wloc_def, state_rel_add_clock])
+  >- (
+   rename [‘eval s (Var vname)’] >>
+   fs [crepSemTheory.eval_def] >> rveq >>
+   pairarg_tac >> fs [] >>
+   fs [compile_exp_def] >> rveq >>
+   fs [nested_seq_def, evaluate_def, find_var_def] >>
+   imp_res_tac locals_rel_intro >>
+   fs [eval_def, state_rel_add_clock])
+  >- (
+   rename [‘eval s (Label fname)’] >>
+   fs [crepSemTheory.eval_def, CaseEq "option"] >> rveq >>
+   pairarg_tac >> fs [compile_exp_def] >> rveq >>
+   fs [nested_seq_def, evaluate_def, find_lab_def] >>
+   cases_on ‘v1’ >> rveq >>
+   imp_res_tac code_rel_intro >>
+   fs [eval_def, set_var_def, domain_lookup, wlab_wloc_def,
+       state_rel_def] >>
+   qexists_tac ‘0’ >> fs [] >>
+   fs [locals_rel_def] >> rw [] >>
+   first_x_assum drule >> fs [] >>
+   strip_tac >> fs [] >>
+   fs [lookup_insert] >>
+   TOP_CASE_TAC >> fs [] >>
+   fs [ctxt_max_def] >>
+   first_x_assum drule >> fs [])
+  >- (
+   rename [‘eval s (Load e)’] >>
+   fs [crepSemTheory.eval_def] >>
+   TOP_CASE_TAC >> fs [] >>
+   TOP_CASE_TAC >> fs [] >>
+   rw [] >>
+   pairarg_tac >> fs [] >>
+   fs [compile_exp_def] >>
+   pairarg_tac >> fs [] >> rveq >>
+   last_x_assum drule_all >>
+   disch_then (qspec_then ‘l’ assume_tac) >>
+   fs [] >> rfs [] >>
+   qexists_tac ‘ck’ >> fs [] >>
+   fs [loopSemTheory.eval_def, wlab_wloc_def] >>
+   fs [crepSemTheory.mem_load_def, loopSemTheory.mem_load_def] >> rveq >>
+   imp_res_tac state_rel_intro >>
+   imp_res_tac mem_rel_intro >>
+   last_x_assum (qspec_then ‘c’ mp_tac) >> fs [])
+  >- (
+   rename [‘eval s (LoadByte e)’] >>
+   fs [crepSemTheory.eval_def] >>
+   TOP_CASE_TAC >> fs [] >>
+   TOP_CASE_TAC >> fs [] >>
+   TOP_CASE_TAC >> fs [] >>
+   rw [] >>
+   pairarg_tac >> fs [] >>
+   fs [compile_exp_def] >>
+   pairarg_tac >> fs [] >> rveq >>
+   last_x_assum drule_all >>
+   disch_then (qspec_then ‘l’ assume_tac) >>
+   fs [] >> rfs [] >>
+   qexists_tac ‘ck’ >> fs [] >>
+   drule evaluate_none_nested_seq_append >>
+   disch_then (qspec_then
+               ‘[Assign tmp'' le'; LoadByte tmp'' 0w tmp'']’ mp_tac) >>
+   strip_tac >> fs [] >>
+   fs [nested_seq_def, loopSemTheory.evaluate_def] >>
+   fs [set_var_def, wlab_wloc_def] >>
+   fs [panSemTheory.mem_load_byte_def, CaseEq "word_lab",
+       wordSemTheory.mem_load_byte_aux_def] >>
+   imp_res_tac mem_rel_intro >>
+   last_x_assum (qspec_then ‘byte_align c’ (mp_tac o GSYM)) >>
+   strip_tac >> fs [] >>
+   last_x_assum (qspec_then ‘byte_align c’ (mp_tac o GSYM)) >>
+   strip_tac >> fs [wlab_wloc_def] >>
+   imp_res_tac state_rel_intro >>
+   fs [eval_def, state_rel_def] >>
+   imp_res_tac compile_exp_temp_ge >>
+   fs [locals_rel_def] >> rw [] >>
+   first_x_assum drule >> fs [] >>
+   strip_tac >> fs [] >>
+   fs [lookup_insert] >>
+   TOP_CASE_TAC >> fs [] >>
+   fs [ctxt_max_def] >>
+   first_x_assum drule >> fs [])
+  >- (
+   rename [‘eval s (LoadGlob gadr)’] >>
+   fs [crepSemTheory.eval_def] >>
+   pairarg_tac >> fs [] >>
+   fs [compile_exp_def] >> rveq >>
+   fs [nested_seq_def, loopSemTheory.evaluate_def] >>
+   fs [eval_def] >>
+   imp_res_tac globals_rel_intro >>
+   fs [state_rel_add_clock])
+  >- (
+   rename [‘eval s (Op op es)’] >>
+   rw [] >>
+   pairarg_tac >> fs [] >>
+   fs [Once compile_exp_def] >> fs [] >>
+   pairarg_tac >> fs [] >> rveq >>
+   (* qexists_tac ‘0’ >> fs [] >> *)
+
+
+   fs [crepSemTheory.eval_def, CaseEq "option"] >> rveq >>
+   fs [loopSemTheory.eval_def] >>
+   ‘∃ck st.
+    evaluate (nested_seq p,t with clock := ck + t.clock) = (NONE,st) ∧
+    the_words (MAP (λa. eval r a) les) =
+    SOME ((MAP (λw. case w of Word n =>  n | Label v1 => ARB) ws))’ by (
+     qpat_x_assum ‘word_op _ _ = _’ kall_tac >>
+     rpt (pop_assum mp_tac) >>
+     MAP_EVERY qid_spec_tac [‘t’, ‘p’, ‘les’ , ‘tmp’, ‘l’,‘ws’, ‘es’] >>
+     Induct
+     >- (
+      rw [] >>
+      fs [OPT_MMAP_def] >> rveq >>
+      fs [compile_exp_def] >> rveq >>
+      fs [nested_seq_def, loopSemTheory.evaluate_def, wordSemTheory.the_words_def]) >>
+     rpt gen_tac >>
+     once_rewrite_tac [compile_exp_def] >>
+     rw [] >> fs [] >>
+     fs [OPT_MMAP_def] >> rveq >>
+     pairarg_tac >> fs [] >>
+     pairarg_tac >> fs [] >> rveq >>
+     first_x_assum (qspec_then ‘h’ mp_tac) >>
+     fs [] >>
+     disch_then drule_all >>
+     disch_then (qspec_then ‘l’ assume_tac) >>
+     fs [] >> rfs [] >>
+     fs [loopSemTheory.evaluate_def] >>
+     last_x_assum (qspecl_then
+                   [‘l''’, ‘tmp''’, ‘les'’, ‘p1’, ‘st’] mp_tac) >>
+     fs [] >>
+     imp_res_tac compile_exp_temp_ge >>
+     fs [] >> strip_tac >> fs [] >>
+     qexists_tac ‘ck’ >>
+     qpat_x_assum ‘evaluate (nested_seq p',_) = (_,_)’ assume_tac >>
+     drule evaluate_none_nested_seq_append >>
+     disch_then (qspec_then ‘p1’ mp_tac) >>
+     strip_tac >> fs [] >>
+
+
+
+
+     impl_tac
+     >- (
+      imp_res_tac evaluate_none_nested_seq_append >>
+      fs []) >>
+     strip_tac >> fs [] >>
+     cases_on ‘h'’ >> fs [] >>
+     fs [wordSemTheory.the_words_def] >>
+     ‘eval r le = eval st le’ suffices_by fs [wlab_wloc_def] >>
+     drule evaluate_nested_seq_append_first >>
+     disch_then drule >>
+     strip_tac >> fs [] >>
+     drule compile_exps_prog_update_locals_clock >>
+     disch_then drule >>
+     strip_tac >>
+     drule nested_seq_pure_evaluation >>
+     disch_then drule >> fs [wlab_wloc_def] >>
+     disch_then (qspecl_then [‘tmp''’, ‘le’, ‘Word c’] mp_tac) >>
+     impl_tac
+     >- (
+      fs [] >>
+      conj_tac >- cheat >>
+      conj_tac >- cheat >>
+      rw [] >>
+      imp_res_tac locals_rel_intro >>
+      drule compile_exp_locals_touched_le_tmp >>
+      disch_then (qspecl_then [‘ctxt’, ‘tmp’, ‘l’, ‘p'’, ‘le’,
+                               ‘tmp''’, ‘l''’, ‘n’] mp_tac) >>
+      fs [] >>
+      impl_tac >- metis_tac [] >> fs []) >>
+     fs []) >>
+
+
+
+
+
+
+
+   ‘t with clock := t.clock = t’ by cheat >> fs [] >>
+   pop_assum kall_tac
+
+
+   cases_on ‘evaluate (nested_seq p,t)’ >> fs [] >>
+   ‘q = NONE /\ the_words (MAP (λa. eval r a) les) =
+    SOME ((MAP (λw. case w of Word n =>  n | Label v1 => ARB) ws))’ by (
+     qpat_x_assum ‘word_op _ _ = _’ kall_tac >>
+     rpt (pop_assum mp_tac) >>
+     MAP_EVERY qid_spec_tac [‘t’, ‘p’, ‘les’ , ‘tmp’, ‘l’,‘ws’, ‘es’] >>
+     Induct
+     >- (
+      rw [] >>
+      fs [OPT_MMAP_def] >> rveq >>
+      fs [compile_exp_def] >> rveq >>
+      fs [nested_seq_def, loopSemTheory.evaluate_def, wordSemTheory.the_words_def]) >>
+     rpt gen_tac >>
+     once_rewrite_tac [compile_exp_def] >>
+     ntac 11 strip_tac >> fs [] >>
+     fs [OPT_MMAP_def] >> rveq >>
+     pairarg_tac >> fs [] >>
+     pairarg_tac >> fs [] >> rveq >>
+     first_x_assum (qspec_then ‘h’ mp_tac) >>
+     fs [] >>
+     disch_then drule_all >>
+     disch_then (qspec_then ‘l’ assume_tac) >>
+     fs [] >> rfs [] >>
+     fs [loopSemTheory.evaluate_def] >>
+     last_x_assum (qspecl_then
+                   [‘l''’, ‘tmp''’, ‘les'’, ‘p1’, ‘st’] mp_tac) >>
+     fs [] >>
+     imp_res_tac compile_exp_temp_ge >>
+     fs [] >>
+     impl_tac
+     >- (
+      imp_res_tac evaluate_none_nested_seq_append >>
+      fs []) >>
+     strip_tac >> fs [] >>
+     cases_on ‘h'’ >> fs [] >>
+     fs [wordSemTheory.the_words_def] >>
+     ‘eval r le = eval st le’ suffices_by fs [wlab_wloc_def] >>
+     drule evaluate_nested_seq_append_first >>
+     disch_then drule >>
+     strip_tac >> fs [] >>
+     drule compile_exps_prog_update_locals_clock >>
+     disch_then drule >>
+     strip_tac >>
+     drule nested_seq_pure_evaluation >>
+     disch_then drule >> fs [wlab_wloc_def] >>
+     disch_then (qspecl_then [‘tmp''’, ‘le’, ‘Word c’] mp_tac) >>
+     impl_tac
+     >- (
+      fs [] >>
+      conj_tac >- cheat >>
+      conj_tac >- cheat >>
+      rw [] >>
+      imp_res_tac locals_rel_intro >>
+      drule compile_exp_locals_touched_le_tmp >>
+      disch_then (qspecl_then [‘ctxt’, ‘tmp’, ‘l’, ‘p'’, ‘le’,
+                               ‘tmp''’, ‘l''’, ‘n’] mp_tac) >>
+      fs [] >>
+      impl_tac >- metis_tac [] >> fs []) >>
+     fs []) >>
+   fs [wlab_wloc_def] >>
+   pop_assum kall_tac >>
+   pop_assum kall_tac >>
+   ntac 8 (pop_assum mp_tac) >>
+   pop_assum kall_tac >>
+   pop_assum kall_tac >>
+   pop_assum mp_tac >>
+   pop_assum mp_tac >>
+   MAP_EVERY qid_spec_tac [‘t’, ‘p’, ‘les’ , ‘tmp’, ‘l’, ‘ws’, ‘es’] >>
+   Induct
+   >- (
+    rw [] >>
+    fs [OPT_MMAP_def] >> rveq >>
+    fs [compile_exp_def] >> rveq >>
+    fs [nested_seq_def, loopSemTheory.evaluate_def, wordSemTheory.the_words_def]) >>
+   rpt gen_tac >>
+   once_rewrite_tac [compile_exp_def] >>
+   ntac 10 strip_tac >> fs [] >>
+   last_x_assum mp_tac >>
+   pairarg_tac >> fs [] >>
+   pairarg_tac >> fs [] >> rveq >>
+   last_x_assum (qspec_then ‘h’ mp_tac) >>
+   fs [] >>
+   fs [OPT_MMAP_def] >> rveq >>
+   disch_then drule_all >>
+   disch_then (qspec_then ‘l’ mp_tac) >>
+   pairarg_tac >> fs [] >> rveq >>
+   strip_tac >> fs [] >>
+   disch_then drule >>
+   disch_then (qspecl_then [‘l''’, ‘tmp''’, ‘les'’, ‘p1’] mp_tac) >>
+   fs [] >>
+   imp_res_tac compile_exp_temp_ge >>
+   fs [] >>
+   imp_res_tac evaluate_nested_seq_append_first >>
+   fs [])
+  >- (
+   rw [] >>
+   fs [crepSemTheory.eval_def, CaseEq "option", CaseEq "word_lab"] >>
+   rveq >> fs [] >>
+   pairarg_tac >> fs [] >>
+   fs [compile_exp_def] >>
+   pairarg_tac >> fs [] >>
+   pairarg_tac >> fs [] >>
+   rveq >> fs [] >>
+   fs [prog_if_def] >>
+   last_x_assum drule_all >>
+   disch_then (qspec_then ‘l’ mp_tac) >>
+   strip_tac >> rfs [] >>
+   last_x_assum (qspecl_then [‘st’, ‘ctxt’, ‘tmp''’, ‘l''’] mp_tac) >>
+   fs [] >>
+   imp_res_tac compile_exp_temp_ge >> fs [] >>
+   strip_tac >> fs [] >>
+   qmatch_goalsub_abbrev_tac ‘nested_seq (_ ++ _ ++ np)’ >>
+
+
+   qpat_x_assum ‘evaluate (_,st) = _’ mp_tac >>
+   drule evaluate_none_nested_seq_append >>
+   disch_then (qspec_then ‘p'' ++ np’ mp_tac) >>
+   strip_tac >> fs [] >>
+   pop_assum kall_tac >>
+   strip_tac >>
+   drule evaluate_none_nested_seq_append >>
+   disch_then (qspec_then ‘np’ mp_tac) >>
+   strip_tac >> fs [] >>
+   pop_assum kall_tac >>
+   fs [Abbr ‘np’, nested_seq_def] >>
+   fs [evaluate_def] >>
+   pairarg_tac >> fs [] >>
+   pairarg_tac >> fs [] >>
+   pairarg_tac >> fs [] >>
+   rfs [] >>
+   ‘eval st' le' = eval st le'’ by (
+     ‘evaluate (nested_seq (p' ++ p''),t) = (NONE,st')’ by
+       metis_tac [evaluate_none_nested_seq_append] >>
+     drule nested_seq_pure_evaluation >>
+     drule_all compile_exp_prog_update_locals_clock >>
+     fs [] >> strip_tac >> fs [wlab_wloc_def] >>
+     disch_then (qspecl_then [‘tmp''’, ‘le'’, ‘Word w1’] mp_tac) >>
+     impl_tac
+     >- (
+      fs [] >>
+      conj_tac >- cheat >>
+      conj_tac >- cheat >>
+      rw [] >>
+      imp_res_tac locals_rel_intro >>
+      dxrule compile_exp_locals_touched_le_tmp >>
+      drule compile_exp_locals_touched_le_tmp >>
+      disch_then (qspecl_then [‘ctxt’, ‘tmp’, ‘l’, ‘p'’, ‘le'’,
+                               ‘tmp''’, ‘l''’, ‘n’] mp_tac) >>
+      fs [] >>
+      impl_tac >- metis_tac [] >> fs []) >>
+     fs []) >>
+   fs [] >> rfs [] >> rveq >>
+   fs [wlab_wloc_def, loopSemTheory.set_var_def,
+       loopSemTheory.eval_def] >>
+   qmatch_goalsub_rename_tac ‘lookup (ftmp + _) _’ >>
+   ‘eval (st' with locals := insert (ftmp + 1) (Word w1) st'.locals)
+    le'' = eval st' le''’ by (
+     ntac 3 (pop_assum kall_tac) >>
+
+
+
+
+cheat
+     ) >>
+   fs [] >> rfs [] >>
+   rveq >>
+   fs [lookup_insert] >>
+   fs [get_var_imm_def] >>
+   cases_on ‘word_cmp cmp w1 w2’ >>
+   fs [loopSemTheory.evaluate_def, loopSemTheory.eval_def,
+       loopSemTheory.set_var_def] >>
+
+
+
+   fs [cut_res_def, cut_state_def] >>
+   fs [AllCaseEqs()]  >> rveq >> fs [] >>
+
+
+
+   ‘domain l'³' ⊆
+    tmp'³' + 1 INSERT tmp'³' + 2 INSERT tmp'³' + 1 INSERT
+    domain st'.locals’ by cheat >>
+   fs [] >>
+   ‘st'.clock <> 0’ by cheat >> fs [] >>
+   rveq >>
+   fs [dec_clock_def] >>
+   fs [lookup_inter_alt] >>
+   conj_tac >> EVAL_TAC >>
+   conj_tac >> fs [state_rel_def]
+
+
+   , cut_state_def]
+
+
+
+
+
+
+
+
+
+
+
+
+
+
+
+
+
+
+
+
+
+
+
+
+
+
+
+
+
+
+Theorem compile_exp_prog_upd_locals_clock_cases:
+  (!ct tmp l (e :α crepLang$exp) p le tmp' l' res s (t :(α, β) state).
+    compile_exp ct tmp l e = (p,le,tmp', l') /\
+    evaluate (nested_seq p,s) = (res,t) ==>
+       t = s with <|locals := t.locals; clock := t.clock|>) /\
+   (!ct tmp l (e :α crepLang$exp list) p le tmp' l' res s (t :(α, β) state).
+    compile_exps ct tmp l e = (p,le,tmp', l') /\
+    evaluate (nested_seq p,s) = (res,t) ==>
+       t = s with <|locals := t.locals; clock := t.clock|>)
+Proof
+  rw []
+  >- (
+   drule compile_exp_comp_syn_ok >>
+   strip_tac >> fs [] >>
+   drule comp_syn_ok_upd_local_clock >> fs []) >>
+  drule compile_exps_comp_syn_ok >>
+  strip_tac >> fs [] >>
+  drule comp_syn_ok_upd_local_clock >> fs []
+QED
+
+val compile_exp_prog_upd_locals_clock = compile_exp_prog_upd_locals_clock_cases |> CONJUNCT1
+val compile_exps_prog_upd_locals_clock = compile_exp_prog_upd_locals_clock_cases |> CONJUNCT2
+
+
+Theorem comp_syn_ok_upd_local_clock:
+  !p s res t.
+    evaluate (p,s) = (res,t) /\
+    comp_syntax_ok p ==>
+     t = s with <|locals := t.locals; clock := t.clock|>
+Proof
+  recInduct evaluate_ind >> rw [] >>
+  TRY (fs [Once comp_syntax_ok_def, every_prog_def] >> NO_TAC)
+  >- (
+   fs [evaluate_def] >> rveq >>
+   fs [state_component_equality])
+  >- (
+   fs [evaluate_def] >>
+   FULL_CASE_TAC >> fs [set_var_def] >>
+   rveq >> fs [state_component_equality])
+  >- (
+   fs [evaluate_def] >>
+   every_case_tac >> fs [set_var_def] >> rveq >>
+   fs [state_component_equality])
+  >- (
+   drule comp_syn_ok_seq >>
+   strip_tac >>
+   fs [evaluate_def] >>
+   pairarg_tac >> fs [] >>
+   FULL_CASE_TAC >> fs []  >> rveq >>
+   fs [state_component_equality])
+  >- (
+   drule comp_syn_ok_if >>
+   strip_tac >>
+   fs [evaluate_def] >>
+   every_case_tac >> fs [] >> rveq >>
+   fs [state_component_equality]
+   >- (
+    cases_on ‘evaluate (c1,s)’ >> fs [] >>
+    fs [cut_res_def, cut_state_def, dec_clock_def] >>
+    every_case_tac >> fs [] >> rveq >> fs []) >>
+   cases_on ‘evaluate (c2,s)’ >> fs [] >>
+   fs [cut_res_def, cut_state_def, dec_clock_def] >>
+   every_case_tac >> fs [] >> rveq >> fs []) >>
+  fs [evaluate_def] >>
+  FULL_CASE_TAC >> fs [set_var_def] >>
+  rveq >> fs [state_component_equality]
+QED
+
+
+
+(* p can have cut_set *)
+
+Theorem unassigned_vars_evaluate_same:
+  !p s res t n.
+   evaluate (p,s) = (res,t) /\
+   (res = NONE ∨ res = SOME Continue ∨ res = SOME Break) /\
+    ~MEM n (assigned_vars p) ==>
+  lookup n t.locals = lookup n s.locals
+Proof
+  cheat
+QED
+
+
+Theorem compile_exp_locals_touched_le_tmp:
+  !s e v ct tmp l p le tmp' l' n.
+   eval s e = SOME v /\
+   ctxt_max ct.vmax ct.vars ∧
+   (∀n v. FLOOKUP s.locals n = SOME v ⇒
+   ∃m. FLOOKUP ct.vars n = SOME m) /\
+   compile_exp ct tmp l e = (p,le,tmp', l') /\
+   ctxt_max ct.vmax ct.vars /\ ct.vmax < tmp /\
+    MEM n (locals_touched le) ==>
+    n < tmp'
+Proof
+  ho_match_mp_tac crepSemTheory.eval_ind >> rw []
+  >- (
+   fs [compile_exp_def] >> rveq >>
+   fs [locals_touched_def])
+  >- (
+   fs [compile_exp_def] >> rveq >>
+   fs [locals_touched_def] >>
+   fs [crepSemTheory.eval_def, find_var_def] >>
+   res_tac >> rfs [] >> fs [] >>
+   rveq >> fs [ctxt_max_def] >>
+   res_tac >> fs [])
+  >- (
+   fs [compile_exp_def] >> rveq >>
+   fs [locals_touched_def])
+  >- (
+   fs [compile_exp_def] >> rveq >>
+   pairarg_tac >> fs [] >> rveq >>
+   fs [crepSemTheory.eval_def, CaseEq "option", CaseEq "word_lab"] >>
+   rveq >> fs [] >>
+   fs [locals_touched_def] >> res_tac >> fs [])
+  >- (
+   fs [compile_exp_def] >> rveq >>
+   pairarg_tac >> fs [] >> rveq >>
+   fs [crepSemTheory.eval_def, CaseEq "option", CaseEq "word_lab"] >>
+   rveq >> fs [locals_touched_def])
+  >- (
+   fs [compile_exp_def] >> rveq >>
+   fs [locals_touched_def])
+  >- (
+   fs [Once compile_exp_def] >> rveq >>
+   pairarg_tac >> fs [] >> rveq >>
+   fs [locals_touched_def] >>
+   fs [crepSemTheory.eval_def, CaseEq "option"] >> rveq >> fs [] >>
+   qpat_x_assum ‘word_op _ _ = _’ kall_tac >>
+   qpat_x_assum ‘EVERY _ _’ kall_tac >>
+   rpt (pop_assum mp_tac) >>
+   MAP_EVERY qid_spec_tac [‘p’, ‘les’ , ‘tmp’, ‘l’,‘ws’, ‘es’] >>
+   Induct
+   >- (
+    rw [] >>
+    fs [OPT_MMAP_def] >> rveq >>
+    fs [compile_exp_def] >> rveq >>
+    fs [nested_seq_def, loopSemTheory.evaluate_def, wordSemTheory.the_words_def]) >>
+   rpt gen_tac >>
+   rw [] >>
+   last_x_assum mp_tac >>
+   impl_tac >- metis_tac [] >>
+   strip_tac >> fs [] >>
+   fs [OPT_MMAP_def] >> rveq >> fs [] >>
+   qpat_x_assum ‘compile_exps _ _ _ _ = _’ mp_tac >>
+   once_rewrite_tac [compile_exp_def] >>
+   fs [] >>
+   strip_tac >> pairarg_tac >> fs [] >>
+   pairarg_tac >> fs [] >> rveq >> fs []
+   >- (
+    last_x_assum (qspec_then ‘h’ mp_tac) >>
+    fs [] >>
+    disch_then drule >>
+    disch_then drule >>
+    fs [] >>
+    disch_then (qspecl_then
+                  [‘tmp’, ‘l’, ‘p'’, ‘le’, ‘tmp''’, ‘l''’, ‘n’] mp_tac) >>
+    fs [] >>
+    strip_tac >> fs [] >>
+    imp_res_tac compile_exps_temp_ge >> fs []) >>
+   rfs [] >>
+   first_x_assum (qspecl_then [‘l''’, ‘tmp''’ , ‘les'’, ‘p1’] mp_tac) >>
+   fs [] >>
+   imp_res_tac compile_exp_temp_ge >> fs [])
+  >- (
+   fs [compile_exp_def] >> rveq >>
+   pairarg_tac >> fs [] >>
+   pairarg_tac >> fs [] >> rveq >> fs [] >>
+   fs [locals_touched_def]) >>
+  fs [crepSemTheory.eval_def, CaseEq "option", CaseEq "word_lab"] >>
+  fs [compile_exp_def] >> rveq >>
+  pairarg_tac >> fs [] >> rveq >> fs [] >>
+  fs [locals_touched_def] >>
+  res_tac >> fs []
+QED
+
+
+Theorem comp_exp_preserves_eval:
+  ∀s e v (t :('a, 'b) state) ctxt tmp l.
+  eval s e = SOME v /\
+  state_rel s t /\ mem_rel ctxt s.memory t.memory /\
+  globals_rel ctxt s.globals t.globals /\
+  code_rel ctxt s.code t.code /\
+  locals_rel ctxt s.locals t.locals /\
+  ctxt.vmax < tmp ==>
+    let (p,le, tmp, l) = compile_exp ctxt tmp l e in
+     ?ck st. evaluate (nested_seq p,t with clock := t.clock + ck) = (NONE,st) /\
+     eval st le = SOME (wlab_wloc ctxt v) /\
+     state_rel s st /\ mem_rel ctxt s.memory st.memory /\
+     globals_rel ctxt s.globals st.globals /\
+     code_rel ctxt s.code st.code /\
+     locals_rel ctxt s.locals st.locals
+Proof
+  ho_match_mp_tac crepSemTheory.eval_ind >>
+  rpt conj_tac >> rpt gen_tac >> strip_tac
+  >- (
+   rename [‘Const w’] >>
+   fs [crepSemTheory.eval_def] >> rveq >>
+   fs [compile_exp_def] >>
+   fs [nested_seq_def, evaluate_def, eval_def, wlab_wloc_def])
+  >- (
+   rename [‘eval s (Var vname)’] >>
+   fs [crepSemTheory.eval_def] >> rveq >>
+   pairarg_tac >> fs [] >>
+   fs [compile_exp_def] >> rveq >>
+   fs [nested_seq_def, evaluate_def, find_var_def] >>
+   imp_res_tac locals_rel_intro >>
+   fs [eval_def])
+  >- (
+   rename [‘eval s (Label fname)’] >>
+   fs [crepSemTheory.eval_def, CaseEq "option"] >> rveq >>
+   pairarg_tac >> fs [compile_exp_def] >> rveq >>
+   fs [nested_seq_def, evaluate_def, find_lab_def] >>
+   cases_on ‘v1’ >> rveq >>
+   imp_res_tac code_rel_intro >>
+   fs [eval_def, set_var_def, domain_lookup, wlab_wloc_def,
+       state_rel_def] >>
+   fs [locals_rel_def] >> rw [] >>
+   first_x_assum drule >> fs [] >>
+   strip_tac >> fs [] >>
+   fs [lookup_insert] >>
+   TOP_CASE_TAC >> fs [] >>
+   fs [ctxt_max_def] >>
+   first_x_assum drule >> fs [])
+  >- (
+   rename [‘eval s (Load e)’] >>
+   fs [crepSemTheory.eval_def] >>
+   TOP_CASE_TAC >> fs [] >>
+   TOP_CASE_TAC >> fs [] >>
+   rw [] >>
+   pairarg_tac >> fs [] >>
+   fs [compile_exp_def] >>
+   pairarg_tac >> fs [] >> rveq >>
+   last_x_assum drule_all >>
+   disch_then (qspec_then ‘l’ assume_tac) >>
+   fs [] >> rfs [] >>
+   fs [loopSemTheory.eval_def, wlab_wloc_def] >>
+   fs [crepSemTheory.mem_load_def, loopSemTheory.mem_load_def] >> rveq >>
+   imp_res_tac state_rel_intro >>
+   imp_res_tac mem_rel_intro >>
+   last_x_assum (qspec_then ‘c’ mp_tac) >> fs [])
+  >- (
+   rename [‘eval s (LoadByte e)’] >>
+   fs [crepSemTheory.eval_def] >>
+   TOP_CASE_TAC >> fs [] >>
+   TOP_CASE_TAC >> fs [] >>
+   TOP_CASE_TAC >> fs [] >>
+   rw [] >>
+   pairarg_tac >> fs [] >>
+   fs [compile_exp_def] >>
+   pairarg_tac >> fs [] >> rveq >>
+   last_x_assum drule_all >>
+   disch_then (qspec_then ‘l’ assume_tac) >>
+   fs [] >> rfs [] >>
+   drule evaluate_none_nested_seq_append >>
+   disch_then (qspec_then
+               ‘[Assign tmp'' le'; LoadByte tmp'' 0w tmp'']’ mp_tac) >>
+   strip_tac >> fs [] >>
+   fs [nested_seq_def, loopSemTheory.evaluate_def] >>
+   fs [set_var_def, wlab_wloc_def] >>
+   fs [panSemTheory.mem_load_byte_def, CaseEq "word_lab",
+       wordSemTheory.mem_load_byte_aux_def] >>
+   imp_res_tac mem_rel_intro >>
+   last_x_assum (qspec_then ‘byte_align c’ (mp_tac o GSYM)) >>
+   strip_tac >> fs [] >>
+   last_x_assum (qspec_then ‘byte_align c’ (mp_tac o GSYM)) >>
+   strip_tac >> fs [wlab_wloc_def] >>
+   imp_res_tac state_rel_intro >>
+   fs [eval_def, state_rel_def] >>
+   imp_res_tac compile_exp_temp_ge >>
+   fs [locals_rel_def] >> rw [] >>
+   first_x_assum drule >> fs [] >>
+   strip_tac >> fs [] >>
+   fs [lookup_insert] >>
+   TOP_CASE_TAC >> fs [] >>
+   fs [ctxt_max_def] >>
+   first_x_assum drule >> fs [])
+  >- (
+   rename [‘eval s (LoadGlob gadr)’] >>
+   fs [crepSemTheory.eval_def] >>
+   pairarg_tac >> fs [] >>
+   fs [compile_exp_def] >> rveq >>
+   fs [nested_seq_def, loopSemTheory.evaluate_def] >>
+   fs [eval_def] >>
+   imp_res_tac globals_rel_intro >>
+   fs [])
+  >- (
+   rename [‘eval s (Op op es)’] >>
+   rw [] >>
+   pairarg_tac >> fs [] >>
+   fs [Once compile_exp_def] >> fs [] >>
+   pairarg_tac >> fs [] >> rveq >>
+   fs [crepSemTheory.eval_def, CaseEq "option"] >> rveq >>
+   fs [loopSemTheory.eval_def] >>
+   cases_on ‘evaluate (nested_seq p,t)’ >> fs [] >>
+   ‘q = NONE /\ the_words (MAP (λa. eval r a) les) =
+    SOME ((MAP (λw. case w of Word n =>  n | Label v1 => ARB) ws))’ by (
+     qpat_x_assum ‘word_op _ _ = _’ kall_tac >>
+     rpt (pop_assum mp_tac) >>
+     MAP_EVERY qid_spec_tac [‘t’, ‘p’, ‘les’ , ‘tmp’, ‘l’,‘ws’, ‘es’] >>
+     Induct
+     >- (
+      rw [] >>
+      fs [OPT_MMAP_def] >> rveq >>
+      fs [compile_exp_def] >> rveq >>
+      fs [nested_seq_def, loopSemTheory.evaluate_def, wordSemTheory.the_words_def]) >>
+     rpt gen_tac >>
+     once_rewrite_tac [compile_exp_def] >>
+     ntac 11 strip_tac >> fs [] >>
+     fs [OPT_MMAP_def] >> rveq >>
+     pairarg_tac >> fs [] >>
+     pairarg_tac >> fs [] >> rveq >>
+     first_x_assum (qspec_then ‘h’ mp_tac) >>
+     fs [] >>
+     disch_then drule_all >>
+     disch_then (qspec_then ‘l’ assume_tac) >>
+     fs [] >> rfs [] >>
+     fs [loopSemTheory.evaluate_def] >>
+     last_x_assum (qspecl_then
+                   [‘l''’, ‘tmp''’, ‘les'’, ‘p1’, ‘st’] mp_tac) >>
+     fs [] >>
+     imp_res_tac compile_exp_temp_ge >>
+     fs [] >>
+     impl_tac
+     >- (
+      imp_res_tac evaluate_none_nested_seq_append >>
+      fs []) >>
+     strip_tac >> fs [] >>
+     cases_on ‘h'’ >> fs [] >>
+     fs [wordSemTheory.the_words_def] >>
+     ‘eval r le = eval st le’ suffices_by fs [wlab_wloc_def] >>
+     drule evaluate_nested_seq_append_first >>
+     disch_then drule >>
+     strip_tac >> fs [] >>
+     drule compile_exps_prog_update_locals_clock >>
+     disch_then drule >>
+     strip_tac >>
+     drule nested_seq_pure_evaluation >>
+     disch_then drule >> fs [wlab_wloc_def] >>
+     disch_then (qspecl_then [‘tmp''’, ‘le’, ‘Word c’] mp_tac) >>
+     impl_tac
+     >- (
+      fs [] >>
+      conj_tac >- cheat >>
+      conj_tac >- cheat >>
+      rw [] >>
+      imp_res_tac locals_rel_intro >>
+      drule compile_exp_locals_touched_le_tmp >>
+      disch_then (qspecl_then [‘ctxt’, ‘tmp’, ‘l’, ‘p'’, ‘le’,
+                               ‘tmp''’, ‘l''’, ‘n’] mp_tac) >>
+      fs [] >>
+      impl_tac >- metis_tac [] >> fs []) >>
+     fs []) >>
+   fs [wlab_wloc_def] >>
+   pop_assum kall_tac >>
+   pop_assum kall_tac >>
+   ntac 8 (pop_assum mp_tac) >>
+   pop_assum kall_tac >>
+   pop_assum kall_tac >>
+   pop_assum mp_tac >>
+   pop_assum mp_tac >>
+   MAP_EVERY qid_spec_tac [‘t’, ‘p’, ‘les’ , ‘tmp’, ‘l’, ‘ws’, ‘es’] >>
+   Induct
+   >- (
+    rw [] >>
+    fs [OPT_MMAP_def] >> rveq >>
+    fs [compile_exp_def] >> rveq >>
+    fs [nested_seq_def, loopSemTheory.evaluate_def, wordSemTheory.the_words_def]) >>
+   rpt gen_tac >>
+   once_rewrite_tac [compile_exp_def] >>
+   ntac 10 strip_tac >> fs [] >>
+   last_x_assum mp_tac >>
+   pairarg_tac >> fs [] >>
+   pairarg_tac >> fs [] >> rveq >>
+   last_x_assum (qspec_then ‘h’ mp_tac) >>
+   fs [] >>
+   fs [OPT_MMAP_def] >> rveq >>
+   disch_then drule_all >>
+   disch_then (qspec_then ‘l’ mp_tac) >>
+   pairarg_tac >> fs [] >> rveq >>
+   strip_tac >> fs [] >>
+   disch_then drule >>
+   disch_then (qspecl_then [‘l''’, ‘tmp''’, ‘les'’, ‘p1’] mp_tac) >>
+   fs [] >>
+   imp_res_tac compile_exp_temp_ge >>
+   fs [] >>
+   imp_res_tac evaluate_nested_seq_append_first >>
+   fs [])
+  >- (
+   rw [] >>
+   fs [crepSemTheory.eval_def, CaseEq "option", CaseEq "word_lab"] >>
+   rveq >> fs [] >>
+   pairarg_tac >> fs [] >>
+   fs [compile_exp_def] >>
+   pairarg_tac >> fs [] >>
+   pairarg_tac >> fs [] >>
+   rveq >> fs [] >>
+   fs [prog_if_def] >>
+   last_x_assum drule_all >>
+   disch_then (qspec_then ‘l’ mp_tac) >>
+   strip_tac >> rfs [] >>
+   last_x_assum (qspecl_then [‘st’, ‘ctxt’, ‘tmp''’, ‘l''’] mp_tac) >>
+   fs [] >>
+   imp_res_tac compile_exp_temp_ge >> fs [] >>
+   strip_tac >> fs [] >>
+   qmatch_goalsub_abbrev_tac ‘nested_seq (_ ++ _ ++ np)’ >>
+
+
+   qpat_x_assum ‘evaluate (_,st) = _’ mp_tac >>
+   drule evaluate_none_nested_seq_append >>
+   disch_then (qspec_then ‘p'' ++ np’ mp_tac) >>
+   strip_tac >> fs [] >>
+   pop_assum kall_tac >>
+   strip_tac >>
+   drule evaluate_none_nested_seq_append >>
+   disch_then (qspec_then ‘np’ mp_tac) >>
+   strip_tac >> fs [] >>
+   pop_assum kall_tac >>
+   fs [Abbr ‘np’, nested_seq_def] >>
+   fs [evaluate_def] >>
+   pairarg_tac >> fs [] >>
+   pairarg_tac >> fs [] >>
+   pairarg_tac >> fs [] >>
+   rfs [] >>
+   ‘eval st' le' = eval st le'’ by (
+     ‘evaluate (nested_seq (p' ++ p''),t) = (NONE,st')’ by
+       metis_tac [evaluate_none_nested_seq_append] >>
+     drule nested_seq_pure_evaluation >>
+     drule_all compile_exp_prog_update_locals_clock >>
+     fs [] >> strip_tac >> fs [wlab_wloc_def] >>
+     disch_then (qspecl_then [‘tmp''’, ‘le'’, ‘Word w1’] mp_tac) >>
+     impl_tac
+     >- (
+      fs [] >>
+      conj_tac >- cheat >>
+      conj_tac >- cheat >>
+      rw [] >>
+      imp_res_tac locals_rel_intro >>
+      dxrule compile_exp_locals_touched_le_tmp >>
+      drule compile_exp_locals_touched_le_tmp >>
+      disch_then (qspecl_then [‘ctxt’, ‘tmp’, ‘l’, ‘p'’, ‘le'’,
+                               ‘tmp''’, ‘l''’, ‘n’] mp_tac) >>
+      fs [] >>
+      impl_tac >- metis_tac [] >> fs []) >>
+     fs []) >>
+   fs [] >> rfs [] >> rveq >>
+   fs [wlab_wloc_def, loopSemTheory.set_var_def,
+       loopSemTheory.eval_def] >>
+   qmatch_goalsub_rename_tac ‘lookup (ftmp + _) _’ >>
+   ‘eval (st' with locals := insert (ftmp + 1) (Word w1) st'.locals)
+    le'' = eval st' le''’ by (
+     ntac 3 (pop_assum kall_tac) >>
+
+
+
+
+cheat
+     ) >>
+   fs [] >> rfs [] >>
+   rveq >>
+   fs [lookup_insert] >>
+   fs [get_var_imm_def] >>
+   cases_on ‘word_cmp cmp w1 w2’ >>
+   fs [loopSemTheory.evaluate_def, loopSemTheory.eval_def,
+       loopSemTheory.set_var_def] >>
+
+
+
+   fs [cut_res_def, cut_state_def] >>
+   fs [AllCaseEqs()]  >> rveq >> fs [] >>
+
+
+
+   ‘domain l'³' ⊆
+    tmp'³' + 1 INSERT tmp'³' + 2 INSERT tmp'³' + 1 INSERT
+    domain st'.locals’ by cheat >>
+   fs [] >>
+   ‘st'.clock <> 0’ by cheat >> fs [] >>
+   rveq >>
+   fs [dec_clock_def] >>
+   fs [lookup_inter_alt] >>
+   conj_tac >> EVAL_TAC >>
+   conj_tac >> fs [state_rel_def]
+
+
+   , cut_state_def]
+
+
+
+
+
+
+
+
+
+
+
+
+
+
+
+   ) >>
+  rw [] >>
+  fs [crepSemTheory.eval_def, CaseEq "option", CaseEq "word_lab"] >>
+  rveq >> fs [] >>
+  pairarg_tac >> fs [compile_exp_def] >>
+  pairarg_tac >> fs [] >> rveq >>
+  fs [loopSemTheory.evaluate_def] >>
+  last_x_assum drule_all >>
+  strip_tac >> rfs [] >>
+  fs [loopSemTheory.eval_def, wlab_wloc_def]
+QED
+
+
+
+
+
+
+
+
+
+QED
+
+
+Theorem nested_seq_pure_evaluation:
+  !s e v t ctxt tmp l p le ntmp nl st q.
+  eval s e = SOME v ∧ state_rel s t ∧ mem_rel ctxt s.memory t.memory ∧
+  globals_rel ctxt s.globals t.globals ∧ code_rel ctxt s.code t.code ∧
+  locals_rel ctxt s.locals t.locals ∧ ctxt.vmax < tmp /\
+  compile_exp ctxt tmp l e = (p,le,ntmp,nl) /\
+  evaluate (nested_seq p, t) = (NONE, st) /\
+  st = t with <|locals := st.locals; clock := st.clock |> /\
+  (!n. MEM n (assigned_vars (nested_seq q)) ==> ntmp <= n) /\
+  (!(st :(α, β) loopSem$state) pt res. evaluate (nested_seq q,st) = (res, pt) ==>
+   res = NONE /\ pt = st with <|locals := pt.locals; clock := pt.clock |>) ==>
+    ?res (nt :(α, β) loopSem$state). evaluate (nested_seq (p ++ q),t) = (res, nt) /\
+    eval nt le = SOME (wlab_wloc ctxt v)
+Proof
+  ho_match_mp_tac crepSemTheory.eval_ind >>
+  rpt conj_tac >> rpt gen_tac >> strip_tac
+  >- (
+   fs [crepSemTheory.eval_def] >>
+   rveq >> fs [] >>
+   fs [compile_exp_def] >>
+   rveq >> fs [] >>
+   cases_on ‘evaluate (nested_seq q,t)’ >>
+   fs [eval_def, wlab_wloc_def])
+  >- (
+   fs [crepSemTheory.eval_def] >>
+   rveq >> fs [] >>
+   fs [compile_exp_def, find_var_def] >>
+   rveq >> fs [] >>
+   cases_on ‘evaluate (nested_seq q,t)’ >>
+   fs [] >>
+   first_x_assum drule >>
+   strip_tac >> fs [] >>
+   imp_res_tac locals_rel_intro >>
+   fs [eval_def] >>
+   drule unassigned_vars_evaluate_same >>
+   fs [] >>
+   disch_then (qspec_then ‘n’ mp_tac) >>
+   fs [] >>
+   impl_tac
+   >- (
+    CCONTR_TAC >> fs [] >>
+    ‘n <= ctxt.vmax’ by (
+      fs [ctxt_max_def] >> res_tac >> fs []) >>
+    ‘n < ntmp’ by DECIDE_TAC >>
+    res_tac >> fs []) >>
+   fs [])
+  >- (
+   fs [crepSemTheory.eval_def, CaseEq "option"] >>
+   rveq >> fs [] >>
+   fs [compile_exp_def] >> rveq >> fs [] >>
+   cases_on ‘v1’ >> fs [] >>
+   imp_res_tac code_rel_intro >> fs [] >>
+   fs [nested_seq_def, evaluate_def,
+       find_lab_def, domain_lookup, set_var_def] >>
+   rveq >> fs [] >>
+   fs [eval_def] >>
+   cases_on ‘evaluate (nested_seq q,t with locals :=
+              insert tmp (Loc loc 0) t.locals)’ >>
+   fs [] >>
+   res_tac >> fs [] >>
+   drule unassigned_vars_evaluate_same >>
+   fs [] >>
+   disch_then (qspec_then ‘tmp’ mp_tac) >>
+   fs [] >>
+   impl_tac
+   >- (
+    CCONTR_TAC >> fs [] >>
+    res_tac >> fs []) >>
+   ‘t with <|locals := insert tmp (Loc loc 0) t.locals;
+    clock := t.clock|> = t with <|locals := insert tmp (Loc loc 0) t.locals|>’ by
+     fs [state_component_equality] >>
+   fs [wlab_wloc_def])
+  >- (
+   rpt gen_tac >>
+   strip_tac >>
+   fs [crepSemTheory.eval_def, CaseEq "option", CaseEq "word_lab"] >>
+   rveq >> fs [] >>
+   fs [compile_exp_def] >> rveq >> fs [] >>
+   pairarg_tac >> fs [] >> rveq >> fs [] >>
+   last_x_assum drule >>
+   disch_then drule_all >>
+   strip_tac >>
+   fs [eval_def, wlab_wloc_def] >>
+   drule evaluate_none_nested_seq_append >>
+   disch_then (qspec_then ‘q’ mp_tac) >>
+   fs [] >> strip_tac >>
+   pop_assum (assume_tac o GSYM) >>
+   res_tac >> fs [] >>
+   fs [mem_load_def, crepSemTheory.mem_load_def] >>
+   fs [Once state_component_equality, state_rel_def, mem_rel_def] >>
+   last_x_assum (qspec_then ‘w’ mp_tac) >> fs [] >>
+   first_x_assum (qspec_then ‘w’ mp_tac) >>
+   fs [])
+  >- cheat
+  >- cheat
+  >- (
+   rpt gen_tac >>
+   strip_tac >>
+   fs [crepSemTheory.eval_def, CaseEq "option"] >>
+   rveq >> fs [] >>
+   fs [Once compile_exp_def] >>
+   pairarg_tac >> fs [] >> rveq >> fs [] >>
+   fs [eval_def] >>
+   cases_on ‘evaluate (nested_seq (p ++ q),t)’ >> fs [] >>
+   ‘the_words (MAP (λa. eval st a) les) =
+    SOME ((MAP (λw. case w of Word n =>  n | Label v1 => ARB) ws))’ by (
+     qpat_x_assum ‘word_op _ _ = _’ kall_tac >>
+     qpat_x_assum ‘∀n. MEM n (assigned_vars (nested_seq q)) ⇒ ntmp <= n’ kall_tac >>
+     pop_assum kall_tac >> pop_assum mp_tac >>
+     pop_assum kall_tac >>
+     strip_tac >>
+     rpt (pop_assum mp_tac) >>
+     MAP_EVERY qid_spec_tac [‘st’, ‘t’, ‘p’, ‘les’ , ‘tmp’, ‘l’,‘ws’, ‘es’] >>
+     Induct
+     >- (
+      rw [] >>
+      fs [OPT_MMAP_def] >> rveq >>
+      fs [compile_exp_def] >> rveq >>
+      fs [nested_seq_def, loopSemTheory.evaluate_def, wordSemTheory.the_words_def]) >>
+     rpt gen_tac >>
+     rpt strip_tac >>
+     fs [OPT_MMAP_def] >> rveq >> fs [] >>
+     qpat_x_assum ‘compile_exps _ _ _ (h::es) = _’ mp_tac >>
+     once_rewrite_tac [compile_exp_def] >>
+     fs [] >> strip_tac >>
+     pairarg_tac >> fs [] >>
+     pairarg_tac >> fs [] >>
+     rveq >> fs [] >>
+     first_x_assum (qspec_then ‘h’ mp_tac) >>
+     fs [] >>
+     disch_then drule >> disch_then drule >>
+     fs [] >>
+     disch_then (qspecl_then [‘tmp’, ‘l’, ‘p'’, ‘le’, ‘tmp'’, ‘l''’] mp_tac) >>
+     fs [] >>
+     cases_on ‘evaluate (nested_seq p',t) = (NONE,st')’ >> fs [] >>
+     disch_then (qspec_then ‘[]’ mp_tac) >>
+     fs [] >>
+     impl_tac
+     >- (
+      conj_tac >- cheat >>
+      fs [nested_seq_def, assigned_vars_def, evaluate_def] >>
+      fs [state_component_equality]) >>
+     strip_tac >>
+
+
+      )
+
+
+
+
+     last_x_assum mp_tac >>
+     impl_tac >- metis_tac [] >>
+     fs [] >>
+     disch_then drule >>
+     fs [] >>
+     disch_then (qspecl_then [‘l''’, ‘tmp'’,
+                              ‘les'’, ‘p1’, ‘st’] mp_tac) >>
+     fs []
+
+
+
+
+
+
+
+     rveq >> rfs [] >>
+     pairarg_tac >> rveq >>
+     first_x_assum (qspec_then ‘h’ mp_tac)>>
+     simp [] >>
+     disch_then (qspecl_then [‘t’, ‘ctxt’] mp_tac) >>
+
+
+     disch_then (qspecl_then [‘tmp’, ‘l’, ‘p'’, ‘le’, ‘tmp'’, ‘l''’] mp_tac) >>
+     simp [] >> fs [] >>
+     pairarg_tac >> fs [] >> rveq >>
+     fs [wordSemTheory.the_words_def] >>
+     cases_on ‘evaluate (nested_seq p', t)’ >>
+     disch_then (qspecl_then [‘p1’, ‘r’, ‘st’] mp_tac) >>
+     impl_tac
+     >- cheat >>
+     strip_tac >> fs [] >>
+     cases_on ‘h'’ >> fs [] >>
+     fs [wlab_wloc_def] >>
+     last_x_assum drule >>
+     fs [] >>
+     disch_then (qspecl_then [‘l''’, ‘tmp'’, ‘les'’, ‘p1’, ‘st’] mp_tac) >>
+     fs [] >>
+     impl_tac >- cheat >>
+     fs []) >>
+
+
+
+
+   )
+
+
+QED
+
+
+
+Theorem nested_seq_pure_evaluation:
+  !s e v t ctxt tmp l p le ntmp nl q st nt.
+  eval s e = SOME v ∧ state_rel s t ∧ mem_rel ctxt s.memory t.memory ∧
+  globals_rel ctxt s.globals t.globals ∧ code_rel ctxt s.code t.code ∧
+  locals_rel ctxt s.locals t.locals ∧ ctxt.vmax < tmp /\
+  compile_exp ctxt tmp l e = (p,le,ntmp,nl) /\
+  (!n. MEM n (assigned_vars (nested_seq q)) ==> ntmp <= n) /\
+  evaluate (nested_seq p, t) = (NONE, st) /\
+  evaluate (nested_seq q,st) = (NONE, nt) /\
+  nt = st with <|locals := nt.locals; clock := nt.clock |> ==>
+  eval nt le = SOME (wlab_wloc ctxt v) /\
+  state_rel s st ∧ mem_rel ctxt s.memory st.memory ∧
+  globals_rel ctxt s.globals st.globals ∧ code_rel ctxt s.code st.code ∧
+  locals_rel ctxt s.locals st.locals
+Proof
+  ho_match_mp_tac crepSemTheory.eval_ind >>
+  rpt conj_tac >> rpt gen_tac >> strip_tac
+  >- (
+   fs [crepSemTheory.eval_def] >>
+   rveq >> fs [] >>
+   fs [compile_exp_def] >>
+   rveq >> fs [] >>
+   fs [nested_seq_def, evaluate_def, eval_def,
+       wlab_wloc_def])
+  >- (
+   fs [crepSemTheory.eval_def] >>
+   rveq >> fs [] >>
+   fs [compile_exp_def, find_var_def] >>
+   rveq >> fs [] >>
+   imp_res_tac locals_rel_intro >>
+   fs [nested_seq_def, evaluate_def] >>
+   rveq >> fs [eval_def] >>
+   drule unassigned_vars_evaluate_same >>
+   fs [] >>
+   disch_then (qspec_then ‘n’ mp_tac) >>
+   fs [] >>
+   impl_tac
+   >- (
+    CCONTR_TAC >> fs [] >>
+    ‘n <= ctxt.vmax’ by (
+      fs [ctxt_max_def] >> res_tac >> fs []) >>
+    ‘n < ntmp’ by DECIDE_TAC >>
+    res_tac >> fs []) >>
+   fs [])
+  >- (
+   fs [crepSemTheory.eval_def, CaseEq "option"] >>
+   rveq >> fs [] >>
+   fs [compile_exp_def] >> rveq >> fs [] >>
+   cases_on ‘v1’ >> fs [] >>
+   imp_res_tac code_rel_intro >> fs [] >>
+   fs [nested_seq_def, evaluate_def,
+       find_lab_def, domain_lookup, set_var_def] >>
+   rveq >> fs [] >>
+   fs [eval_def] >>
+   drule unassigned_vars_evaluate_same >>
+   fs [] >>
+   disch_then (qspec_then ‘tmp’ mp_tac) >>
+   fs [] >>
+   impl_tac
+   >- (
+    CCONTR_TAC >> fs [] >>
+    res_tac >> fs []) >>
+   fs [wlab_wloc_def] >>
+   strip_tac >>
+   conj_tac >- fs [state_rel_def] >>
+   fs [locals_rel_def] >>
+   rw [] >>
+   fs [ctxt_max_def] >>
+   first_x_assum drule >>
+   strip_tac >> fs [] >>
+   last_x_assum drule >>
+   fs [lookup_insert])
+  >- (
+   rpt gen_tac >>
+   strip_tac >>
+   last_x_assum mp_tac >>
+   fs [crepSemTheory.eval_def, CaseEq "option", CaseEq "word_lab"] >>
+   rveq >> fs [] >>
+   fs [Once compile_exp_def] >> rveq >> fs [] >>
+   pairarg_tac >> fs [] >> rveq >> fs [] >>
+   fs [eval_def] >>
+   disch_then drule_all >>
+   strip_tac >> fs [wlab_wloc_def] >>
+   drule_all compile_exp_prog_update_locals_clock >>
+   strip_tac >> fs [] >>
+   fs [mem_load_def, crepSemTheory.mem_load_def] >>
+   fs [Once state_component_equality, state_rel_def, mem_rel_def] >>
+   last_x_assum (qspec_then ‘w’ mp_tac) >> fs [] >>
+   first_x_assum (qspec_then ‘w’ mp_tac) >>
+   fs [])
+  >- (
+   rpt gen_tac >>
+   strip_tac >>
+   last_x_assum mp_tac >>
+   fs [crepSemTheory.eval_def, CaseEq "option", CaseEq "word_lab"] >>
+   rveq >> fs [] >>
+   fs [Once compile_exp_def] >> rveq >> fs [] >>
+   pairarg_tac >> fs [] >> rveq >> fs [] >>
+   fs [eval_def] >>
+   cases_on ‘evaluate (nested_seq p',t)’ >>
+   reverse (cases_on ‘q'’) >> fs []
+   >- (
+    drule evaluate_not_none_nested_seq_append >>
+    disch_then (qspec_then ‘[Assign tmp' le'; LoadByte tmp' 0w tmp']’ mp_tac) >>
+    fs []) >>
+   disch_then (qspecl_then [‘t’, ‘ctxt’, ‘tmp’, ‘l’, ‘p'’, ‘le'’, ‘tmp'’, ‘l'’] mp_tac) >>
+   disch_then (qspecl_then [‘[]’, ‘r’, ‘r’] mp_tac) >>
+   fs [] >>
+   impl_tac
+   >- (
+    conj_tac
+    >- (
+     rw [] >>
+     fs [nested_seq_def] >>
+     fs [assigned_vars_def] >> res_tac >> fs []) >>
+    fs [state_component_equality, nested_seq_def, evaluate_def]) >>
+   strip_tac >> fs [] >>
+   ‘lookup tmp' st.locals = SOME (wlab_wloc ctxt (Word (w2w w')))’ by (
+     drule_all evaluate_nested_seq_append_first >>
+     fs [] >> strip_tac >>
+     fs [nested_seq_def, evaluate_def] >>
+     pairarg_tac >> fs [] >>
+     pairarg_tac >> fs [] >>
+     cases_on ‘eval r le'’ >> fs [] >> rveq >> fs [] >>
+     fs [set_var_def, lookup_insert, wlab_wloc_def] >>
+     imp_res_tac state_rel_intro >> fs [] >>
+     fs [wordSemTheory.mem_load_byte_aux_def,
+         panSemTheory.mem_load_byte_def] >>
+     imp_res_tac mem_rel_intro >>
+     last_x_assum (qspec_then ‘byte_align w’ mp_tac) >>
+     strip_tac >> fs [] >>
+     cases_on ‘s.memory (byte_align w)’ >> fs [wlab_wloc_def] >>
+     pop_assum mp_tac >> pop_assum (assume_tac o GSYM) >>
+     fs [] >> rfs [] >> rveq >> fs [] >>
+     fs [state_component_equality] >>
+     qpat_x_assum ‘_ = st.locals’ (assume_tac o GSYM) >>
+     fs []) >>
+   fs [] >>
+   drule_all evaluate_nested_seq_append_first >>
+   fs [nested_seq_def, evaluate_def] >>
+   pairarg_tac >> fs [] >>
+   fs [set_var_def, lookup_insert] >>
+   fs [wlab_wloc_def] >>
+   imp_res_tac state_rel_intro >> fs [] >>
+   fs [wordSemTheory.mem_load_byte_aux_def,
+       panSemTheory.mem_load_byte_def] >>
+   imp_res_tac mem_rel_intro >>
+   last_x_assum (qspec_then ‘byte_align w’ mp_tac) >>
+   strip_tac >> fs [] >>
+   cases_on ‘s.memory (byte_align w)’ >> fs [wlab_wloc_def] >>
+   pop_assum mp_tac >> pop_assum (assume_tac o GSYM) >>
+   fs [] >> rfs [] >> rveq >> fs [] >>
+   strip_tac >> strip_tac >>
+   fs [] >> rveq >> fs [] >>
+   dxrule unassigned_vars_evaluate_same >>
+   drule unassigned_vars_evaluate_same >>
+   fs [] >>
+   disch_then (qspec_then ‘tmp'’ assume_tac) >>
+   strip_tac >>
+   pop_assum kall_tac >> fs [] >>
+   pop_assum mp_tac >> fs [] >>
+   impl_tac
+   >- (
+    CCONTR_TAC >> fs [] >>
+    res_tac >> fs []) >>
+   fs [] >> strip_tac >> fs [] >>
+   fs [state_rel_def] >>
+   fs [locals_rel_def] >>
+   rw [] >>
+   fs [ctxt_max_def] >>
+   first_x_assum drule >>
+   strip_tac >> fs [] >>
+   first_x_assum drule >>
+   strip_tac >> fs [] >>
+   drule compile_exp_temp_ge >>
+   strip_tac >>
+   fs [lookup_insert])
+  >- (
+   fs [crepSemTheory.eval_def] >>
+   rveq >> fs [] >>
+   fs [compile_exp_def] >>
+   rveq >> fs [] >>
+   fs [nested_seq_def, evaluate_def, eval_def,
+       wlab_wloc_def] >>
+   imp_res_tac globals_rel_intro >>
+   res_tac >> fs [] >> rveq >>
+   fs [state_component_equality])
+  >- (
+   rpt gen_tac >>
+   strip_tac >>
+   last_x_assum mp_tac >>
+   fs [crepSemTheory.eval_def, CaseEq "option"] >>
+   rveq >> fs [] >>
+   fs [Once compile_exp_def] >>
+   pairarg_tac >> fs [] >> rveq >> fs [] >>
+   fs [eval_def] >>
+   strip_tac >>
+   ‘the_words (MAP (λa. eval st a) les) =
+    SOME ((MAP (λw. case w of Word n =>  n | Label v1 => ARB) ws))’ by (
+     qpat_x_assum ‘word_op _ _ = _’ kall_tac >>
+     qpat_x_assum ‘∀n. MEM n (assigned_vars (nested_seq q)) ⇒ ntmp <= n’ kall_tac >>
+     qpat_x_assum ‘evaluate (nested_seq q,st) = (NONE,nt)’ kall_tac >>
+     rpt (pop_assum mp_tac) >>
+     MAP_EVERY qid_spec_tac [‘st’, ‘t’, ‘p’, ‘les’ , ‘tmp’, ‘l’,‘ws’, ‘es’] >>
+     Induct
+     >- (
+      rw [] >>
+      fs [OPT_MMAP_def] >> rveq >>
+      fs [compile_exp_def] >> rveq >>
+      fs [nested_seq_def, loopSemTheory.evaluate_def, wordSemTheory.the_words_def]) >>
+     rpt gen_tac >>
+     ntac 12 strip_tac >>
+
+
+
+
+
+     qpat_x_assum ‘OPT_MMAP _ (_::_) = _’ mp_tac >>
+     simp [OPT_MMAP_def] >>
+     strip_tac >>  rveq >>
+     qpat_x_assum ‘compile_exps _ _ _ (h::es) = _’ mp_tac >>
+     once_rewrite_tac [compile_exp_def] >>
+     simp [] >>
+     strip_tac >> rveq >> rfs [] >>
+     pairarg_tac >> rveq >>
+     first_x_assum (qspec_then ‘h’ mp_tac)>>
+     simp [] >>
+     disch_then (qspecl_then [‘t’, ‘ctxt’] mp_tac) >>
+
+
+     disch_then (qspecl_then [‘tmp’, ‘l’, ‘p'’, ‘le’, ‘tmp'’, ‘l''’] mp_tac) >>
+     simp [] >> fs [] >>
+     pairarg_tac >> fs [] >> rveq >>
+     fs [wordSemTheory.the_words_def] >>
+     cases_on ‘evaluate (nested_seq p', t)’ >>
+     disch_then (qspecl_then [‘p1’, ‘r’, ‘st’] mp_tac) >>
+     impl_tac
+     >- cheat >>
+     strip_tac >> fs [] >>
+     cases_on ‘h'’ >> fs [] >>
+     fs [wlab_wloc_def] >>
+     last_x_assum drule >>
+     fs [] >>
+     disch_then (qspecl_then [‘l''’, ‘tmp'’, ‘les'’, ‘p1’, ‘st’] mp_tac) >>
+     fs [] >>
+     impl_tac >- cheat >>
+     fs []) >>
+
+
+
+
+      )
+
+
+     last_x_assum drule >>
+     fs [] >>
+     disch_then (qspecl_then [‘l''’, ‘tmp'’, ‘les'’, ‘p1’, ‘q’] mp_tac) >>
+     fs []
+
+
+
+
+
+
+     impl_tac
+     >- (
+
+
+
+      )
+
+nt = st
+
+     cheat) >>
+   fs [] >>
+
+
+
+
+
+
+
+
+
+
+
+
+
+
+
+
+
+
+
+
+
+
+
+
+
+
+
+
+
+
+
+
+
+
+
+     ) >>
+   fs [] >>
+
+
+
+
+   )
+
+
+
+
+
+
+
+
+
+Theorem foo:
+  ∀s e v (t :('a, 'b) state) ctxt tmp l.
+  eval s e = SOME v /\
+  state_rel s t /\ mem_rel ctxt s.memory t.memory /\
+  globals_rel ctxt s.globals t.globals /\
+  code_rel ctxt s.code t.code /\
+  locals_rel ctxt s.locals t.locals /\
+  ctxt.vmax < tmp  ==>
+    let (p,le, tmp, l) = compile_exp ctxt tmp l e in
+     ?st. evaluate (nested_seq p,t) = (NONE,st) /\
+     eval st le = SOME (wlab_wloc ctxt v) /\
+     state_rel s st /\ mem_rel ctxt s.memory st.memory /\
+     globals_rel ctxt s.globals st.globals /\
+     code_rel ctxt s.code st.code /\
+     locals_rel ctxt s.locals st.locals
+Proof
+  ho_match_mp_tac crepSemTheory.eval_ind >>
+  rpt conj_tac >> rpt gen_tac >> strip_tac
+  >- (
+   rename [‘Const w’] >>
+   fs [crepSemTheory.eval_def] >> rveq >>
+   fs [compile_exp_def] >>
+   fs [nested_seq_def, evaluate_def, eval_def, wlab_wloc_def])
+  >- (
+   rename [‘eval s (Var vname)’] >>
+   fs [crepSemTheory.eval_def] >> rveq >>
+   pairarg_tac >> fs [] >>
+   fs [compile_exp_def] >> rveq >>
+   fs [nested_seq_def, evaluate_def, find_var_def] >>
+   imp_res_tac locals_rel_intro >>
+   fs [eval_def])
+  >- (
+   rename [‘eval s (Label fname)’] >>
+   fs [crepSemTheory.eval_def, CaseEq "option"] >> rveq >>
+   pairarg_tac >> fs [compile_exp_def] >> rveq >>
+   fs [nested_seq_def, evaluate_def, find_lab_def] >>
+   cases_on ‘v1’ >> rveq >>
+   imp_res_tac code_rel_intro >>
+   fs [eval_def, set_var_def, domain_lookup, wlab_wloc_def,
+       state_rel_def] >>
+   fs [locals_rel_def] >> rw [] >>
+   first_x_assum drule >> fs [] >>
+   strip_tac >> fs [] >>
+   fs [lookup_insert] >>
+   TOP_CASE_TAC >> fs [] >>
+   fs [ctxt_max_def] >>
+   first_x_assum drule >> fs [])
+  >- (
+   rename [‘eval s (Load e)’] >>
+   fs [crepSemTheory.eval_def] >>
+   TOP_CASE_TAC >> fs [] >>
+   TOP_CASE_TAC >> fs [] >>
+   rw [] >>
+   pairarg_tac >> fs [] >>
+   fs [compile_exp_def] >>
+   pairarg_tac >> fs [] >> rveq >>
+   last_x_assum drule_all >>
+   disch_then (qspec_then ‘l’ assume_tac) >>
+   fs [] >> rfs [] >>
+   fs [loopSemTheory.eval_def, wlab_wloc_def] >>
+   fs [crepSemTheory.mem_load_def, loopSemTheory.mem_load_def] >> rveq >>
+   imp_res_tac state_rel_intro >>
+   imp_res_tac mem_rel_intro >>
+   last_x_assum (qspec_then ‘c’ mp_tac) >> fs [])
+  >- (
+   rename [‘eval s (LoadByte e)’] >>
+   fs [crepSemTheory.eval_def] >>
+   TOP_CASE_TAC >> fs [] >>
+   TOP_CASE_TAC >> fs [] >>
+   TOP_CASE_TAC >> fs [] >>
+   rw [] >>
+   pairarg_tac >> fs [] >>
+   fs [compile_exp_def] >>
+   pairarg_tac >> fs [] >> rveq >>
+   last_x_assum drule_all >>
+   disch_then (qspec_then ‘l’ assume_tac) >>
+   fs [] >> rfs [] >>
+   drule evaluate_none_nested_seq_append >>
+   disch_then (qspec_then
+               ‘[Assign tmp'' le'; LoadByte tmp'' 0w tmp'']’ mp_tac) >>
+   strip_tac >> fs [] >>
+   fs [nested_seq_def, loopSemTheory.evaluate_def] >>
+   fs [set_var_def, wlab_wloc_def] >>
+   fs [panSemTheory.mem_load_byte_def, CaseEq "word_lab",
+       wordSemTheory.mem_load_byte_aux_def] >>
+   imp_res_tac mem_rel_intro >>
+   last_x_assum (qspec_then ‘byte_align c’ (mp_tac o GSYM)) >>
+   strip_tac >> fs [] >>
+   last_x_assum (qspec_then ‘byte_align c’ (mp_tac o GSYM)) >>
+   strip_tac >> fs [wlab_wloc_def] >>
+   imp_res_tac state_rel_intro >>
+   fs [eval_def, state_rel_def] >>
+   imp_res_tac compile_exp_temp_ge >>
+   fs [locals_rel_def] >> rw [] >>
+   first_x_assum drule >> fs [] >>
+   strip_tac >> fs [] >>
+   fs [lookup_insert] >>
+   TOP_CASE_TAC >> fs [] >>
+   fs [ctxt_max_def] >>
+   first_x_assum drule >> fs [])
+  >- (
+   rename [‘eval s (LoadGlob gadr)’] >>
+   fs [crepSemTheory.eval_def] >>
+   pairarg_tac >> fs [] >>
+   fs [compile_exp_def] >> rveq >>
+   fs [nested_seq_def, loopSemTheory.evaluate_def] >>
+   fs [eval_def] >>
+   imp_res_tac globals_rel_intro >>
+   fs [])
+  >- (
+   rename [‘eval s (Op op es)’] >>
+   rw [] >>
+   pairarg_tac >> fs [] >>
+   fs [Once compile_exp_def] >> fs [] >>
+   pairarg_tac >> fs [] >> rveq >>
+   fs [crepSemTheory.eval_def, CaseEq "option"] >> rveq >>
+   fs [loopSemTheory.eval_def] >>
+   cases_on ‘evaluate (nested_seq p,t)’ >> fs [] >>
+   ‘q = NONE /\ the_words (MAP (λa. eval r a) les) =
+    SOME ((MAP (λw. case w of Word n =>  n | Label v1 => ARB) ws))’ by (
+     qpat_x_assum ‘word_op _ _ = _’ kall_tac >>
+     rpt (pop_assum mp_tac) >>
+     MAP_EVERY qid_spec_tac [‘t’, ‘p’, ‘les’ , ‘tmp’, ‘l’,‘ws’, ‘es’] >>
+     Induct
+     >- (
+      rw [] >>
+      fs [OPT_MMAP_def] >> rveq >>
+      fs [compile_exp_def] >> rveq >>
+      fs [nested_seq_def, loopSemTheory.evaluate_def, wordSemTheory.the_words_def]) >>
+     rpt gen_tac >>
+     once_rewrite_tac [compile_exp_def] >>
+     ntac 11 strip_tac >> fs [] >>
+     fs [OPT_MMAP_def] >> rveq >>
+     pairarg_tac >> fs [] >>
+     pairarg_tac >> fs [] >> rveq >>
+     first_x_assum (qspec_then ‘h’ mp_tac) >>
+     fs [] >>
+     disch_then drule_all >>
+     disch_then (qspec_then ‘l’ assume_tac) >>
+     fs [] >> rfs [] >>
+     fs [loopSemTheory.evaluate_def] >>
+     last_x_assum (qspecl_then
+                   [‘l''’, ‘tmp''’, ‘les'’, ‘p1’, ‘st’] mp_tac) >>
+     fs [] >>
+     imp_res_tac compile_exp_temp_ge >>
+     fs [] >>
+     impl_tac
+     >- (
+      imp_res_tac evaluate_none_nested_seq_append >>
+      fs []) >>
+     strip_tac >> fs [] >>
+     cases_on ‘h'’ >> fs [] >>
+     fs [wordSemTheory.the_words_def] >>
+     ‘eval r le = eval st le’ suffices_by fs [wlab_wloc_def] >>
+     drule isit >>
+     disch_then (qspecl_then [‘t’, ‘ctxt’, ‘tmp’] mp_tac) >>
+     fs [] >>
+     disch_then drule >>
+     disch_then (qspecl_then [‘p1’, ‘st’, ‘r’] mp_tac) >>
+     fs [] >>
+     impl_tac >- cheat >>
+     fs []) >>
+   fs [wlab_wloc_def] >>
+   pop_assum kall_tac >>
+   pop_assum kall_tac >>
+   ntac 8 (pop_assum mp_tac) >>
+   pop_assum kall_tac >>
+   pop_assum kall_tac >>
+   pop_assum mp_tac >>
+   pop_assum mp_tac >>
+   MAP_EVERY qid_spec_tac [‘t’, ‘p’, ‘les’ , ‘tmp’, ‘l’, ‘ws’, ‘es’] >>
+   Induct
+   >- (
+    rw [] >>
+    fs [OPT_MMAP_def] >> rveq >>
+    fs [compile_exp_def] >> rveq >>
+    fs [nested_seq_def, loopSemTheory.evaluate_def, wordSemTheory.the_words_def]) >>
+   rpt gen_tac >>
+   once_rewrite_tac [compile_exp_def] >>
+   ntac 10 strip_tac >> fs [] >>
+   last_x_assum mp_tac >>
+   pairarg_tac >> fs [] >>
+   pairarg_tac >> fs [] >> rveq >>
+   last_x_assum (qspec_then ‘h’ mp_tac) >>
+   fs [] >>
+   fs [OPT_MMAP_def] >> rveq >>
+   disch_then drule_all >>
+   disch_then (qspec_then ‘l’ mp_tac) >>
+   pairarg_tac >> fs [] >> rveq >>
+   strip_tac >> fs [] >>
+   disch_then drule >>
+   disch_then (qspecl_then [‘l''’, ‘tmp''’, ‘les'’, ‘p1’] mp_tac) >>
+   fs [] >>
+   imp_res_tac compile_exp_temp_ge >>
+   fs [] >>
+   imp_res_tac evaluate_nested_seq_append_first >>
+   fs [])
+
+
+       compile_exp ct tmp l ce = (prog,le,ntmp,nl) /\
+  evaluate (nested_seq prog,s) = (NONE,st) /\
+  eval st le = SOME w /\
+  (!n. MEM n (assigned_vars prog') ==> ntmp <= n)
+
+
+
+
+  evaluate (nested_seq q,st) = (res, nt) /\
+  res = NONE /\ nt = st with locals := nt.locals ==>
+  evaluate (nested_seq (p ++ q), s) = (NONE, nt) /\
+   eval nt e = SOME w
+Proof
+
+QED
+
+eval cexp cs = SOME w
+  compile_exp cexp tmp = (prog, lexp, tmp') ==>
+  ?...
+    evaluate (prog ++ prog', s) = (NONE, s') /\
+    eval lexp s' = SOME (convert w)
+  lexp -- only reads from vars < tmp'
+  prog' -- only assigns to vars >= tmp'
+  prog' -- only touches the locals part of state
+
+
+
+fs []
+  evaluate (prog ++ prog', s) = (NONE, s') /\
+    eval lexp s' = SOME (convert w)
+
+
+
+  prog =unseq p p'
+       evaluate p t = st
+       evaluate p' st = r
+
+       le:les
+
+
+     ‘eval r le = eval st le’ by (
+       pop_assum kall_tac >>
+       qpat_x_assum ‘T’ kall_tac >>
+       qpat_x_assum ‘EVERY _ _’ kall_tac >>
+       rpt (pop_assum mp_tac) >>
+       MAP_EVERY qid_spec_tac [‘t’, ‘p1’, ‘st’,‘les'’ ,‘tmp'’, ‘l'’,
+                               ‘tmp''’, ‘l''’, ‘t'’, ‘es’] >>
+       Induct
+       >- (
+        rw [] >>
+        fs [compile_exp_def] >> rveq >>
+        fs [evaluate_def] >> rveq >> fs []) >>
+       rw [] >>
+       rfs [] >>
+       fs [OPT_MMAP_def] >> rveq >> fs [] >>
+       qpat_x_assum ‘compile_exps _ _ _ _ = _ ’ mp_tac >>
+       once_rewrite_tac [compile_exp_def] >>
+       fs [] >>
+       pairarg_tac >> fs [] >>
+       pairarg_tac >> fs [] >>
+       strip_tac >> fs [] >> rveq >>
+       first_x_assum drule >>
+       disch_then drule >>
+       fs [] >>
+       strip_tac >>
+
+
+
+
+
+
+
+
+
+
+
+
+
+
+
+
+
+
+
+
+
+
+
+
+
+
+
+
+
+
+
+
+
+
+
+
+
+
+
+
+Theorem abc:
+  !ct tmp l e ps les ntmp nl i t.
+   compile_exp ct tmp l e = (ps, les, ntmp, nl) /\
+   i < LENGTH ps ==>
+     let (q,st) = evaluate (nested_seq (TAKE i ps),t);
+         (r, nt)  = evaluate (EL i ps, st) in
+         st.globals = nt.globals
+Proof
+  qsuff_tac ‘(!ct tmp l (e :α crepLang$exp) ps les ntmp nl i t.
+               compile_exp ct tmp l e = (ps, les, ntmp, nl) /\
+               i < LENGTH ps==>
+               let (q,st:(α, β) state) = evaluate (nested_seq (TAKE i ps),t);
+               (r, nt)  = evaluate (EL i ps, st) in
+               st.globals = nt.globals) /\
+             (!ct tmp l (es :α crepLang$exp list) ps les ntmp nl i t.
+               compile_exps ct tmp l es = (ps, les, ntmp, nl) /\
+                i < LENGTH ps ==>
+                let (q,st:(α, β) state) = evaluate (nested_seq (TAKE i ps),t);
+                (r, nt)  = evaluate (EL i ps, st) in
+                st.globals = nt.globals)’
+  >- metis_tac [] >>
+  ho_match_mp_tac compile_exp_ind >> rw []
+  >- (
+   TRY (rpt (pairarg_tac >> fs [])) >>
+   fs [compile_exp_def] >> rveq >> fs [] >>
+   cases_on ‘i’ >> fs [] >>
+   fs [nested_seq_def, evaluate_def])
+  >- (
+   TRY (rpt (pairarg_tac >> fs [])) >>
+   fs [compile_exp_def] >> rveq >> fs [] >>
+   cases_on ‘i’ >> fs [] >>
+   fs [nested_seq_def, evaluate_def])
+  >- (
+   TRY (rpt (pairarg_tac >> fs [])) >>
+   fs [compile_exp_def] >> rveq >> fs [] >>
+   cases_on ‘i’ >> fs [] >>
+   fs [nested_seq_def, evaluate_def] >>
+   every_case_tac >> fs [set_var_def] >> rveq >> fs [])
+  >- (
+   TRY (rpt (pairarg_tac >> fs [])) >>
+   fs [compile_exp_def] >>
+   pairarg_tac >> fs [] >> rveq >> fs [] >>
+   last_x_assum (qspec_then ‘i’ mp_tac) >>
+   fs [] >>
+   disch_then (qspec_then ‘t’ mp_tac) >>
+   pairarg_tac >> fs []) >>
+  >- (
+   TRY (rpt (pairarg_tac >> fs [])) >>
+   fs [compile_exp_def] >>
+   pairarg_tac >> fs [] >> rveq >> fs [] >>
+   ‘p <> []’ by cheat >>
+   fs [] >>
+   cases_on ‘i < LENGTH p’ >> fs []
+   >- (
+    last_x_assum (qspec_then ‘i’ mp_tac) >>
+    fs [] >>
+    ‘i - LENGTH p = 0’ by fs [] >>
+    fs [] >>
+    dxrule TAKE_APPEND1 >>
+    disch_then (qspec_then ‘[Assign tmp' le; LoadByte tmp' 0w tmp']’ mp_tac) >>
+    strip_tac >> fs [] >>
+    disch_then (qspec_then ‘t’ mp_tac) >>
+    fs [EL_APPEND_EQN]) >>
+   fs [NOT_LESS] >>
+   cases_on ‘LENGTH p = i’ >> fs []
+   >- (
+    ‘EL i (p ++ [Assign tmp' le; LoadByte tmp' 0w tmp']) =
+     Assign tmp' le’ by fs [EL_APPEND_EQN] >>
+    fs [evaluate_def, CaseEq "option", set_var_def] >> rveq >> fs []) >>
+   ‘EL i (p ++ [Assign tmp' le; LoadByte tmp' 0w tmp']) =
+    LoadByte tmp' 0w tmp'’ by (
+     fs [EL_APPEND_EQN] >>
+     ‘i - LENGTH p = 1’ by fs [] >>
+     fs []) >>
+   fs [evaluate_def, CaseEq "option", CaseEq "word_loc",
+       set_var_def] >> rveq >> fs [])
+  >- (
+   TRY (rpt (pairarg_tac >> fs [])) >>
+   fs [compile_exp_def] >> rveq >> fs [] >>
+   cases_on ‘i’ >> fs [] >>
+   fs [nested_seq_def, evaluate_def] >>
+   every_case_tac >> fs [set_var_def] >> rveq >> fs [])
+  >- (
+   pairarg_tac >> fs [] >>
+   pairarg_tac >> fs [] >>
+   qpat_x_assum ‘compile_exp _ _ _ _ = _’ mp_tac >>
+   once_rewrite_tac [compile_exp_def] >>
+   strip_tac >> fs [] >>
+   pairarg_tac >> fs [] >> rveq >> fs [] >>
+   last_x_assum (qspec_then ‘i’ mp_tac) >>
+   fs [] >>
+   disch_then (qspec_then ‘t’ mp_tac) >>
+   fs [])
+  >- (
+   pairarg_tac >> fs [] >>
+   pairarg_tac >> fs [] >>
+   fs [compile_exp_def] >>
+   pairarg_tac >> fs [] >>
+   pairarg_tac >> fs [] >>
+   rveq >> fs [] >>
+   fs [prog_if_def] >>
+   ‘p <> [] ∧ p' <> []’ by cheat >>
+   fs [] >>
+   cases_on ‘i < LENGTH p’ >> fs []
+   >- (
+    first_x_assum (qspec_then ‘i’ mp_tac) >>
+    fs [] >>
+    ‘i - LENGTH p = 0’ by fs [] >>
+    fs [] >>
+    dxrule TAKE_APPEND1 >>
+    disch_then (qspec_then ‘p' ++
+                 [Assign (tmp'' + 1) le; Assign (tmp'' + 2) le';
+                  If cmp (tmp'' + 1) (Reg (tmp'' + 2))
+                    (Assign (tmp'' + 1) (Const 1w))
+                    (Assign (tmp'' + 1) (Const 0w))
+                    (insert (tmp'' + 1) () l'')]’ mp_tac) >>
+    strip_tac >> fs [] >>
+    disch_then (qspec_then ‘t’ mp_tac) >>
+    fs [EL_APPEND_EQN]) >>
+   fs [NOT_LESS] >>
+   cases_on ‘i <= LENGTH (p ++ p')’
+   >- (
+    dxrule TAKE_APPEND1 >>
+    disch_then (qspec_then ‘
+                 [Assign (tmp'' + 1) le; Assign (tmp'' + 2) le';
+                  If cmp (tmp'' + 1) (Reg (tmp'' + 2))
+                  (Assign (tmp'' + 1) (Const 1w))
+                  (Assign (tmp'' + 1) (Const 0w))
+                  (insert (tmp'' + 1) () l'')]’ mp_tac) >>
+    strip_tac >> fs [] >>
+
+
+
+
+
+   )
+
+
+   cases_on ‘i’ >> fs []
+   >- (
+    fs [nested_seq_def, evaluate_def] >>
+    rveq >> fs [] >>
+    cases_on ‘p’ >> fs [] >>
+    fs [evaluate_def] >>
+    every_case_tac >> fs [set_var_def] >> rveq >> fs []
+
+    )
+
+
+   disch_then (qspec_then ‘t’ mp_tac) >>
+   pairarg_tac >> fs [])
+
+   rveq >> rfs [])
+
+
+
+
+  >- fs [compile_exp_def]
+  >- fs [compile_exp_def]
+QED
+
+
+(*
+Definition prog_comp_def:
+  (prog_comp ct tmp l [] = []) /\
+  (prog_comp ct tmp l (e::es) =
+   let (p, le, tmp, l) = compile_exp ct tmp l e in
+     p :: prog_comp ct tmp l es)
+End
+
+
+Theorem compile_exps_prog_seq:
+  !es ct tmp l.
+   ?les tmp' l'.
+   compile_exps ct tmp l es = (nested_seq (prog_comp ct tmp l es),les,tmp', l')
+Proof
+  Induct >> rw []
+  >- fs [compile_exp_def, nested_seq_def, prog_comp_def] >>
+  once_rewrite_tac [compile_exp_def] >>
+  fs [] >>
+  pairarg_tac >> fs [] >>
+  pairarg_tac >> fs [] >>
+  fs [] >>
+  fs [prog_comp_def] >>
+  fs [nested_seq_def] >>
+  last_x_assum (qspecl_then [‘ct’, ‘tmp'’, ‘l'’] mp_tac) >>
+  fs []
+QED
+*)
+
+
+
+
+
+
+  rw [] >>
+  pairarg_tac >> fs [] >>
+  pairarg_tac >> fs [] >>
+  ‘LENGTH es = LENGTH les’ by cheat >>
+  match_mp_tac locals_touched_eq_eval_eq >>
+  conj_tac
+  >- (
+   rpt (pop_assum mp_tac) >>
+   MAP_EVERY qid_spec_tac [‘q’,‘t’,‘l’,‘l'’, ‘tmp'’, ‘ctxt’,‘tmp’, ‘n’, ‘p’, ‘st’,
+                           ‘r’,‘nt’,  ‘les’, ‘es’] >>
+   Induct
+   >- (
+    rw [] >> fs [compile_exp_def] >>
+    rveq >> fs []) >>
+   rw [] >>
+   cases_on ‘les’ >> fs [] >>
+
+
+
+   )
+
+
+
+     Theorem abc:
+  !ctxt tmp l e ps les ntmp nl i.
+   compile_exp ctxt tmp l e = (ps, les, ntmp, nl) /\
+   i <= LENGTH ps ==>
+     let (q,st) = evaluate (nested_seq (TAKE i ps),t);
+         (r, nt)  = evaluate (nested_seq (DROP i ps), st) in
+         st.globals = nt.globals
+Proof
+  rw [] >>
+  pairarg_tac >> fs [] >>
+  pairarg_tac >> fs [] >>
+  ‘LENGTH es = LENGTH les’ by cheat >>
+  match_mp_tac locals_touched_eq_eval_eq >>
+  conj_tac
+  >- (
+   rpt (pop_assum mp_tac) >>
+   MAP_EVERY qid_spec_tac [‘q’,‘t’,‘l’,‘l'’, ‘tmp'’, ‘ctxt’,‘tmp’, ‘n’, ‘p’, ‘st’,
+                           ‘r’,‘nt’,  ‘les’, ‘es’] >>
+   Induct
+   >- (
+    rw [] >> fs [compile_exp_def] >>
+    rveq >> fs []) >>
+   rw [] >>
+   cases_on ‘les’ >> fs [] >>
+
+
+
+   )
+
+
+
+
+     Theorem abc:
+  !es ctxt tmp l p les tmp' l' n t.
+   compile_exps ctxt tmp l es = (p, les, tmp', l') /\
+   n < LENGTH les ==>
+     let (q,st) = evaluate (nested_seq (TAKE (n + 1) p),t);
+         (r, nt)  = evaluate (nested_seq (DROP (n + 1) p), st) in
+         eval st (EL n les) = eval nt (EL n les)
+Proof
+  rw [] >>
+  pairarg_tac >> fs [] >>
+  pairarg_tac >> fs [] >>
+  ‘LENGTH es = LENGTH les’ by cheat >>
+  match_mp_tac locals_touched_eq_eval_eq >>
+  conj_tac
+  >- (
+   rpt (pop_assum mp_tac) >>
+   MAP_EVERY qid_spec_tac [‘q’,‘t’,‘l’,‘l'’, ‘tmp'’, ‘ctxt’,‘tmp’, ‘n’, ‘p’, ‘st’,
+                           ‘r’,‘nt’,  ‘les’, ‘es’] >>
+   Induct
+   >- (
+    rw [] >> fs [compile_exp_def] >>
+    rveq >> fs []) >>
+   rw [] >>
+   cases_on ‘les’ >> fs [] >>
+
+
+
+   )
+
+
+
+
+(*
+
+  eval cexp cs = SOME w
+  compile_exp cexp tmp = (prog, lexp, tmp') ==>
+  ?...
+    evaluate (prog ++ prog', s) = (NONE, s') /\
+    eval lexp s' = SOME (convert w)
+
+
+  lexp -- only reads from vars < tmp'
+  prog' -- only assigns to vars >= tmp'
+  prog' -- only touches the locals part of state
+
+
+  compile_exp cexp tmp liveset = (prog, lexp, tmp', liveset') ==>
+  only_reads_from_lower tmp' prog /\
+  only assigns_to_ge tmp prog (also liveset) /\
+  subspt liveset liveset'
+
+
+  compile_exp .. = (ps, ...) ==> prop is true for ps
+  prop is true for ps ==>
+  ps
+
+*)
+
+
+
+Theorem abc:
+  !es ctxt tmp l p les tmp' l' n t.
+   compile_exps ctxt tmp l es = (p, les, tmp', l') /\
+   n < LENGTH les ==>
+     let (a,inst) = evaluate (nested_seq (TAKE n p),t);
+         (b, nst) = evaluate (nested_seq (TAKE (n + 1) p),inst);
+         (c, nist) = evaluate (nested_seq (TAKE (n + 1) p),t);
+         (d, fist)  = evaluate (nested_seq (DROP (n + 1) p), nist) in
+         eval nst (EL n les) = eval fist (EL n les)
+Proof
+  rw [] >>
+  pairarg_tac >> fs [] >>
+  pairarg_tac >> fs [] >>
+  pairarg_tac >> fs [] >>
+  pairarg_tac >> fs [] >>
+  match_mp_tac locals_touched_eq_eval_eq >>
+  conj_tac >-
+
+
+
+  Induct >> rw []
+  >- (
+   fs [compile_exp_def] >>
+   rveq >> fs []) >>
+  qpat_x_assum ‘compile_exps _ _ _ _ = _’ mp_tac >>
+  once_rewrite_tac [compile_exp_def] >>
+  fs [] >>
+  pairarg_tac >> fs [] >>
+  pairarg_tac >> fs [] >>
+  strip_tac >> rveq >> fs [] >>
+  cases_on ‘n’ >> fs []
+  >- (
+   fs [nested_seq_def] >>
+   fs [evaluate_def] >>
+   pairarg_tac >> fs [] >>
+   pairarg_tac >> fs [] >>
+   pairarg_tac >> fs [] >>
+   match_mp_tac locals_touched_eq_eval_eq >> cheat) >>
+  fs [nested_seq_def] >>
+  fs [evaluate_def] >>
+  pairarg_tac >> fs [] >>
+  pairarg_tac >> fs [] >>
+  pairarg_tac >> fs [] >>
+  pairarg_tac >> fs [] >>
+
+
+  last_x_assum mp_tac >>
+  disch_then drule_all >>
+  disch_then (qspecl_then [‘s1’] mp_tac) >>
+  fs [] >>
+  ‘res = NONE’ by cheat >> fs [] >> rveq >> fs []
+  ‘res' = NONE’ by cheat >> fs [] >>
+  fs [ADD1] >>
+  pairarg_tac >> fs [] >>
+  strip_tac >> fs []
+
+
+  disch_then (qspecl_then [‘ctxt’, ‘tmp''’, ‘l''’, ‘p1’, ‘les'’, ‘tmp'’, ‘l'’] mp_tac) >>
+  fs []
+
+
+
+
+
+
+
+
+
+
+
+   ) >>
+
+
+
+   )
+
+
+
+QED
+
+Theorem foo:
+  ∀s e v (t :('a, 'b) state) ctxt tmp l.
+  eval s e = SOME v /\
+  state_rel s t /\ mem_rel ctxt s.memory t.memory /\
+  globals_rel ctxt s.globals t.globals /\
+  code_rel ctxt s.code t.code /\
+  locals_rel ctxt s.locals t.locals /\
+  ctxt.vmax < tmp  ==>
+    let (p,le, tmp, l) = compile_exp ctxt tmp l e in
+      ?st. evaluate (nested_seq p,t) = (NONE,st) /\ eval st le = SOME (wlab_wloc ctxt v) /\
+    state_rel s st /\ mem_rel ctxt s.memory st.memory /\
+    globals_rel ctxt s.globals st.globals /\
+    code_rel ctxt s.code st.code /\
+    locals_rel ctxt s.locals st.locals
+Proof
+  ho_match_mp_tac crepSemTheory.eval_ind >>
+  rpt conj_tac >> rpt gen_tac >> strip_tac
+  >- (
+   rename [‘Const w’] >>
+   fs [crepSemTheory.eval_def] >> rveq >>
+   fs [compile_exp_def] >>
+   fs [evaluate_def, eval_def, wlab_wloc_def])
+  >- (
+   rename [‘eval s (Var vname)’] >>
+   fs [crepSemTheory.eval_def] >> rveq >>
+   pairarg_tac >> fs [] >>
+   fs [compile_exp_def] >> rveq >>
+   fs [evaluate_def, find_var_def] >>
+   imp_res_tac locals_rel_intro >>
+   fs [eval_def])
+  >- (
+   rename [‘eval s (Label fname)’] >>
+   fs [crepSemTheory.eval_def, CaseEq "option"] >> rveq >>
+   pairarg_tac >> fs [compile_exp_def] >> rveq >>
+   fs [evaluate_def, find_lab_def] >>
+   cases_on ‘v1’ >> rveq >>
+   imp_res_tac code_rel_intro >>
+   fs [eval_def, set_var_def, domain_lookup, wlab_wloc_def,
+       state_rel_def] >>
+   fs [locals_rel_def] >> rw [] >>
+   first_x_assum drule >> fs [] >>
+   strip_tac >> fs [] >>
+   fs [lookup_insert] >>
+   TOP_CASE_TAC >> fs [] >>
+   fs [ctxt_max_def] >>
+   first_x_assum drule >> fs [])
+  >- (
+   rename [‘eval s (Load e)’] >>
+   fs [crepSemTheory.eval_def] >>
+   TOP_CASE_TAC >> fs [] >>
+   TOP_CASE_TAC >> fs [] >>
+   rw [] >>
+   pairarg_tac >> fs [] >>
+   fs [compile_exp_def] >>
+   pairarg_tac >> fs [] >> rveq >>
+   last_x_assum drule_all >>
+   disch_then (qspec_then ‘l’ assume_tac) >>
+   fs [] >> rfs [] >>
+   fs [loopSemTheory.eval_def, wlab_wloc_def] >>
+   fs [crepSemTheory.mem_load_def, loopSemTheory.mem_load_def] >> rveq >>
+   imp_res_tac state_rel_intro >>
+   imp_res_tac mem_rel_intro >>
+   last_x_assum (qspec_then ‘c’ mp_tac) >> fs [])
+  >- (
+   rename [‘eval s (LoadByte e)’] >>
+   fs [crepSemTheory.eval_def] >>
+   TOP_CASE_TAC >> fs [] >>
+   TOP_CASE_TAC >> fs [] >>
+   TOP_CASE_TAC >> fs [] >>
+   rw [] >>
+   pairarg_tac >> fs [] >>
+   fs [compile_exp_def] >>
+   pairarg_tac >> fs [] >> rveq >>
+   last_x_assum drule_all >>
+   disch_then (qspec_then ‘l’ assume_tac) >>
+   fs [] >> rfs [] >>
+   fs [loopSemTheory.evaluate_def] >>
+   fs [set_var_def, wlab_wloc_def] >>
+   fs [panSemTheory.mem_load_byte_def, CaseEq "word_lab",
+       wordSemTheory.mem_load_byte_aux_def] >>
+   imp_res_tac mem_rel_intro >>
+   last_x_assum (qspec_then ‘byte_align c’ (mp_tac o GSYM)) >>
+   strip_tac >> fs [] >>
+   last_x_assum (qspec_then ‘byte_align c’ (mp_tac o GSYM)) >>
+   strip_tac >> fs [wlab_wloc_def] >>
+   imp_res_tac state_rel_intro >>
+   fs [eval_def, state_rel_def] >>
+   imp_res_tac compile_exp_temp_ge >>
+   fs [locals_rel_def] >> rw [] >>
+   first_x_assum drule >> fs [] >>
+   strip_tac >> fs [] >>
+   fs [lookup_insert] >>
+   TOP_CASE_TAC >> fs [] >>
+   fs [ctxt_max_def] >>
+   first_x_assum drule >> fs [])
+  >- (
+   rename [‘eval s (LoadGlob gadr)’] >>
+   fs [crepSemTheory.eval_def] >>
+   pairarg_tac >> fs [] >>
+   fs [compile_exp_def] >> rveq >>
+   fs [loopSemTheory.evaluate_def] >>
+   fs [eval_def] >>
+   imp_res_tac globals_rel_intro >>
+   fs [])
+  >- (
+   rename [‘eval s (Op op es)’] >>
+   rw [] >>
+   pairarg_tac >> fs [] >>
+   fs [Once compile_exp_def] >> fs [] >>
+   pairarg_tac >> fs [] >> rveq >>
+   fs [crepSemTheory.eval_def, CaseEq "option"] >> rveq >>
+   fs [loopSemTheory.eval_def] >>
+   ‘LENGTH les = LENGTH es’ by cheat >>
+   (* cases_on ‘evaluate (p,t)’ >> fs [] >> *)
+
+   ‘!n. n < LENGTH les ==>
+     eval
+     (SND (evaluate (nested_seq (TAKE (n+1) p'),
+      SND (evaluate (nested_seq (TAKE n p'), t))))) (EL n les) =
+     eval
+     (SND (evaluate (nested_seq (DROP (n+1) p'),
+      SND (evaluate (nested_seq (TAKE (n+1) p'), t)))))
+     (EL n les)’ by (
+     qpat_x_assum ‘EVERY _ _’ kall_tac >>
+     qpat_x_assum ‘word_op _ _ = _ ’ kall_tac >>
+     rpt (pop_assum mp_tac) >>
+     MAP_EVERY qid_spec_tac [‘ctxt’, ‘s’,‘t’, ‘p'’, ‘tmp'’, ‘tmp’,
+                             ‘l'’,‘l’, ‘ws’, ‘es’, ‘les’] >>
+     Induct
+     >- rw [] >>
+     rw [] >>
+
+
+
+     cases_on ‘n’ >> fs []
+     >- (
+      fs [nested_seq_def, evaluate_def]
+
+
+      )
+
+
+     match_mp_tac eval_states_eq >>
+
+
+     strip_tac
+
+     last_x_assum mp_tac >>
+     disch_then drule >>
+     disch_then drule >>
+     disch_then drule >>
+
+     impl_tac >- metis_tac [] >>
+
+     cases_on ‘n’ >> fs []
+     >- (
+      cases_on ‘es’ >> fs [] >>
+      qpat_x_assum ‘compile_exps _ _ _ _ = _’ mp_tac >>
+      once_rewrite_tac [compile_exp_def] >>
+      fs [] >>
+      pairarg_tac >> fs [] >>
+      pairarg_tac >> fs [] >>
+      strip_tac >> rveq >> fs [] >>
+      fs [nested_seq_def, evaluate_def] >>
+      pairarg_tac >> fs [] >>
+      first_x_assum (qspec_then ‘h'’ mp_tac) >>
+      fs [] >>
+      fs [OPT_MMAP_def] >> fs [] >>
+      disch_then drule_all >>
+      disch_then (qspec_then ‘l’ mp_tac) >>
+      pairarg_tac >> fs [] >>
+      rveq >> fs [] >>
+      strip_tac >> fs [] >>
+      last_x_assum mp_tac >>
+      disch_then (qspecl_then [‘t'’, ‘t''’, ‘l''’, ‘l'’, ‘tmp''’, ‘tmp'’,
+                               ‘p1’, ‘s1’ ,‘s’, ‘ctxt’] mp_tac) >>
+      fs []
+
+         impl_tac >- cheat >>
+
+
+
+
+      )
+
+
+
+      fs [OPT_MMAP_def] >> rveq >>
+      fs [compile_exp_def] >> rveq >>
+      fs [loopSemTheory.evaluate_def, wordSemTheory.the_words_def]) >>
+
+
+
+
+  (* length les = length es *)
+
+
+
+
+
+
+
+
+   ‘q = NONE /\
+    the_words (MAP (λa. eval r a) les) =
+    SOME ((MAP (λw. case w of Word n =>  n | Label v1 => ARB) ws))’ by (
+     qpat_x_assum ‘word_op _ _ = _’ kall_tac >>
+     rpt (pop_assum mp_tac) >>
+     MAP_EVERY qid_spec_tac [‘t’, ‘p’, ‘les’ , ‘tmp’, ‘l’,‘ws’, ‘es’] >>
+     Induct
+     >- (
+      rw [] >>
+      fs [OPT_MMAP_def] >> rveq >>
+      fs [compile_exp_def] >> rveq >>
+      fs [loopSemTheory.evaluate_def, wordSemTheory.the_words_def]) >>
+     rpt gen_tac >>
+     once_rewrite_tac [compile_exp_def] >>
+     ntac 11 strip_tac >> fs [] >>
+     fs [OPT_MMAP_def] >> rveq >>
+     pairarg_tac >> fs [] >>
+     pairarg_tac >> fs [] >> rveq >>
+     first_x_assum (qspec_then ‘h’ mp_tac) >>
+     fs [] >>
+     disch_then drule_all >>
+     disch_then (qspec_then ‘l’ assume_tac) >>
+     fs [] >> rfs [] >>
+     fs [loopSemTheory.evaluate_def] >>
+     last_x_assum (qspecl_then
+                   [‘l''’, ‘tmp''’, ‘les'’, ‘p1’, ‘st’] mp_tac) >>
+     fs [] >>
+     imp_res_tac compile_exp_temp_ge >>
+     fs [] >>
+     strip_tac >> fs [] >>
+     cases_on ‘h'’ >> fs [] >>
+     fs [wordSemTheory.the_words_def] >>
+
+  prog =unseq p p'
+       evaluate p t = st
+       evaluate p' st = r
+
+       le:les
+
+
+     ‘eval r le = eval st le’ by (
+       pop_assum kall_tac >>
+       qpat_x_assum ‘T’ kall_tac >>
+       qpat_x_assum ‘EVERY _ _’ kall_tac >>
+       rpt (pop_assum mp_tac) >>
+       MAP_EVERY qid_spec_tac [‘t’, ‘p1’, ‘st’,‘les'’ ,‘tmp'’, ‘l'’,
+                               ‘tmp''’, ‘l''’, ‘t'’, ‘es’] >>
+       Induct
+       >- (
+        rw [] >>
+        fs [compile_exp_def] >> rveq >>
+        fs [evaluate_def] >> rveq >> fs []) >>
+       rw [] >>
+       rfs [] >>
+       fs [OPT_MMAP_def] >> rveq >> fs [] >>
+       qpat_x_assum ‘compile_exps _ _ _ _ = _ ’ mp_tac >>
+       once_rewrite_tac [compile_exp_def] >>
+       fs [] >>
+       pairarg_tac >> fs [] >>
+       pairarg_tac >> fs [] >>
+       strip_tac >> fs [] >> rveq >>
+       first_x_assum drule >>
+       disch_then drule >>
+       fs [] >>
+       strip_tac >>
+
+
+
+
+
+
+
+
+
+
+
+
+
+
+
+
+
+
+
+ eval st le = SOME (wlab_wloc ctxt (Word c))
+       evaluate (p',t) = (NONE,st)
+        evaluate (p1,st) = (NONE,r)
+
+  compile_exp ctxt tmp l h = (p',le,tmp'',l'') /\
+   compile_exps ctxt tmp'' l'' es = (p1,les',tmp',l')
+
+
+
+
+
+
+
+
+
+
+       ) >>
+     fs [wlab_wloc_def]) >>
+   fs [wlab_wloc_def] >>
+   pop_assum kall_tac >>
+   pop_assum kall_tac >>
+   ntac 8 (pop_assum mp_tac) >>
+   pop_assum kall_tac >>
+   pop_assum kall_tac >>
+   pop_assum mp_tac >>
+   pop_assum mp_tac >>
+   MAP_EVERY qid_spec_tac [‘t’, ‘p’, ‘les’ , ‘tmp’, ‘l’, ‘ws’, ‘es’] >>
+   Induct
+   >- (
+    rw [] >>
+    fs [OPT_MMAP_def] >> rveq >>
+    fs [compile_exp_def] >> rveq >>
+    fs [loopSemTheory.evaluate_def, wordSemTheory.the_words_def]) >>
+   rpt gen_tac >>
+   once_rewrite_tac [compile_exp_def] >>
+   ntac 10 strip_tac >> fs [] >>
+   last_x_assum mp_tac >>
+   pairarg_tac >> fs [] >>
+   pairarg_tac >> fs [] >> rveq >>
+   fs [loopSemTheory.evaluate_def] >>
+   pairarg_tac >> fs [] >>
+   cases_on ‘res’ >> fs [] >>
+   last_x_assum (qspec_then ‘h’ mp_tac) >>
+   fs [] >>
+   fs [OPT_MMAP_def] >> rveq >>
+   disch_then drule_all >>
+   disch_then (qspec_then ‘l’ mp_tac) >>
+   pairarg_tac >> fs [] >> rveq >>
+   strip_tac >> fs [] >>
+   disch_then (qspecl_then
+               [‘l''’, ‘tmp''’, ‘les'’, ‘p1’, ‘s1’] mp_tac) >>
+   fs [] >>
+   imp_res_tac compile_exp_temp_ge >> fs [])
+  >- (
+   rw [] >>
+   fs [crepSemTheory.eval_def, CaseEq "option", CaseEq "word_lab"] >>
+   rveq >> fs [] >>
+   pairarg_tac >> fs [] >>
+   fs [compile_exp_def] >>
+   pairarg_tac >> fs [] >>
+   pairarg_tac >> fs [] >>
+   rveq >> fs [] >>
+   fs [prog_if_def] >>
+   last_x_assum drule_all >>
+   disch_then (qspec_then ‘l’ mp_tac) >>
+   strip_tac >> rfs [] >>
+   last_x_assum (qspecl_then [‘st’, ‘ctxt’, ‘tmp''’, ‘l''’] mp_tac) >>
+   fs [] >>
+   imp_res_tac compile_exp_temp_ge >> fs [] >>
+   strip_tac >> fs [] >>
+   fs [nested_seq_def, loopSemTheory.evaluate_def] >>
+   pairarg_tac >> fs [] >>
+   pairarg_tac >> fs [] >>
+   pairarg_tac >> fs [] >>
+   rfs [] >>
+   ‘eval st' le' = eval st le'’ by cheat >>
+   fs [] >> rfs [] >> rveq >>
+   fs [wlab_wloc_def, loopSemTheory.set_var_def,
+       loopSemTheory.eval_def] >>
+   ‘eval (st' with locals := insert (tmp'³' + 1) (Word w1) st'.locals)
+    le'' = eval st' le''’ by cheat >>
+   fs [] >> rfs [] >>
+   rveq >>
+   fs [lookup_insert] >>
+   fs [get_var_imm_def] >>
+   cases_on ‘word_cmp cmp w1 w2’ >>
+   fs [loopSemTheory.evaluate_def, loopSemTheory.eval_def,
+       loopSemTheory.set_var_def] >>
+
+
+
+   fs [cut_res_def, cut_state_def]
+
+‘domain l'³' ⊆
+             tmp'³' + 1 INSERT tmp'³' + 2 INSERT tmp'³' + 1 INSERT
+             domain st'.locals’ by cheat >>
+   fs [] >>
+   ‘st'.clock <> 0’ by cheat >> fs [] >>
+   rveq >>
+   fs [dec_clock_def] >>
+   fs [lookup_inter_alt] >>
+   conj_tac >> EVAL_TAC >>
+   conj_tac >> fs [state_rel_def]
+
+
+   , cut_state_def]
+
+
+
+
+
+
+
+
+
+
+
+
+
+
+
+   ) >>
+  rw [] >>
+  fs [crepSemTheory.eval_def, CaseEq "option", CaseEq "word_lab"] >>
+  rveq >> fs [] >>
+  pairarg_tac >> fs [compile_exp_def] >>
+  pairarg_tac >> fs [] >> rveq >>
+  fs [loopSemTheory.evaluate_def] >>
+  last_x_assum drule_all >>
+  strip_tac >> rfs [] >>
+  fs [loopSemTheory.eval_def, wlab_wloc_def]
+QED
+
+Theorem compile_Assign:
+  ^(get_goal "compile_prog _ (crepLang$Assign _ _)")
+Proof
+  rpt gen_tac >>
+  rpt strip_tac >>
+  fs [crepSemTheory.evaluate_def] >>
+  fs [CaseEq "option"] >> rveq >> fs [] >>
+  fs [compile_prog_def] >>
+  imp_res_tac locals_rel_intro >>
+  fs [] >>
+  pairarg_tac >> fs [] >>
+  fs [evaluate_def] >>
+  pairarg_tac >> fs [] >>
+
+
+
+
+  TOP_CASE_TAC >> fs []
+  >- (
+   fs [lo] >>
+
+   )
+
+
+  fs [evaluate_def] >>
+  pairarg_tac >> fs [] >>
+
+
+
+
+QED
+
+
 
 
 Theorem foo:
@@ -555,20 +4381,300 @@ QED
 QED
 
 
-Theorem compile_Assign:
-  ^(get_goal "compile_prog _ (crepLang$Assign _ _)")
+
+(*
+
+(*
+ let (p, les, tmp) = compile_exps ctxt tmp [e;e'] in
+   (Seq p (Seq (Assign tmp le) (Assign (tmp + 1) le'))
+        (If cmp tmp (Reg (tmp + 1))
+         (Assign (tmp + 1) (Const 1w)) (Assign (tmp + 1) (Const 0w)) LN)
+*)
+
+
+(compile_exp ctxt tmp (Op bop es) =
+ let (p, les, tmp) = compile_exps ctxt tmp es in
+     (p, Op bop les, tmp)
+
+(compile_exps ctxt tmp [] = (Skip, [], tmp))
+(compile_exps ctxt tmp (e::es) =
+ let (p, le, tmp) = compile_exp ctxt tmp e in
+ let (p1, les, tmp) = compile_exps ctxt tmp es in
+     (Seq p p1, le::les, tmp)
+
+ (Skip, [], tmp))
+
+
+
+  (compile_exp ctxt ((Const c):'a crepLang$exp) =
+   Assign (ctxt.vmax + 1) ((Const c): 'a loopLang$exp)) /\
+  (compile_exp ctxt (Var vname) = Assign (ctxt.vmax + 1)
+   (case FLOOKUP ctxt.vars vname of
+     | SOME n => Var n
+     | NONE => Var 0)) /\
+  (compile_exp ctxt (Label fname) = LocValue (ctxt.vmax + 1)
+   (case FLOOKUP ctxt.funcs fname of
+     | SOME (n, _) => n
+     | NONE => 0)) /\
+  (compile_exp ctxt (Load adr) =
+   Seq (compile_exp ctxt adr)
+       (Assign (ctxt.vmax + 1) (Load (Var (ctxt.vmax + 1))))) /\
+  (compile_exp ctxt (LoadByte adr) =
+   Seq (compile_exp ctxt adr)
+       (LoadByte (ctxt.vmax + 1) 0w (ctxt.vmax + 1))) /\
+  (compile_exp ctxt (LoadGlob gadr) = Assign (ctxt.vmax + 1) (Lookup gadr)) /\
+
+  (compile_exp ctxt (Op bop es) =
+   Seq (comp_assigns (λc e. compile_exp c e) ctxt es)
+       (Assign (ctxt.vmax + 1) (Op bop (load_exps (ctxt.vmax + 1) (LENGTH es))))) /\
+
+
+  (compile_exp ctxt (Cmp cmp e e') =
+   Seq (Seq (compile_exp ctxt e) (compile_exp (ctxt with vmax := ctxt.vmax + 1) e'))
+        (If cmp (ctxt.vmax + 1) (Reg (ctxt.vmax + 2))
+           (Assign (ctxt.vmax + 1) (Const 1w)) (Assign (ctxt.vmax + 1) (Const 0w)) LN)) /\
+  (compile_exp ctxt (Shift sh e n) =
+   Seq (compile_exp ctxt e)
+   (Assign (ctxt.vmax + 1) (Shift sh (Var (ctxt.vmax + 1)) n)))
+Termination
+  cheat
+End
+*)
+
+
+Definition comp_assigns_def:
+  (comp_assigns f ctxt [] =  Skip) /\
+  (comp_assigns f ctxt (e::es) =
+   Seq (f ctxt e)
+       (comp_assigns f (ctxt with vmax := ctxt.vmax + 1) es))
+End
+
+
+Definition load_exps_def:
+  load_exps n m  = MAP Var (GENLIST (λx. n + x) m)
+End
+
+
+
+
+Definition compile_exp_def:
+  (compile_exp ctxt tmp l ((Const c):'a crepLang$exp) = (Skip, Const c, tmp, l)) /\
+  (compile_exp ctxt tmp l (Var v) = (Skip, Var (find_var ctxt v), tmp, l)) /\
+  (compile_exp ctxt tmp l (Label f) = (LocValue tmp (find_lab ctxt f), Var tmp, tmp + 1, l)) /\
+  (compile_exp ctxt tmp l (Load ad) =
+   let (p, le, tmp, l) = compile_exp ctxt tmp l ad in (p, Load le, tmp, l)) /\
+  (compile_exp ctxt tmp l (LoadByte ad) =
+   let (p, le, tmp, l) = compile_exp ctxt tmp l ad in
+    (Seq (Seq p (Assign tmp le)) (LoadByte tmp 0w tmp), Var tmp, tmp + 1, l)) /\
+  (compile_exp ctxt tmp l (LoadGlob gadr) = (Skip, Lookup gadr, tmp, l)) /\
+  (compile_exp ctxt tmp l (Op bop es) =
+   let (p, les, tmp, l) = compile_exps ctxt tmp l es in
+    (p, Op bop les, tmp, l)) /\
+  (compile_exp ctxt tmp l (Cmp cmp e e') =
+   let (p, le, tmp, l) = compile_exp ctxt tmp l e in
+   let (p', le', tmp', l) = compile_exp ctxt tmp l e' in
+    (prog_if cmp p p' le le' (tmp' + 1) (tmp' + 2) l, Var (tmp' + 1), tmp' + 3, insert (tmp' + 1) () l)) /\
+  (compile_exp ctxt tmp l (Shift sh e n) =
+   let (p, le, tmp, l) = compile_exp ctxt tmp l e in (p, Shift sh le n, tmp, l)) /\
+
+  (compile_exps ctxt tmp l [] = (Skip, [], tmp, l)) /\
+  (compile_exps ctxt tmp l (e::es) =
+    let (p, le, tmp, l) = compile_exp ctxt tmp l e in
+    let (p1, les, tmp, l) = compile_exps ctxt tmp l es in
+        (Seq p p1, le::les, tmp, l))
+End
+(*
+Definition toNumSet_def:
+  toNumSet [] = LN ∧
+  toNumSet (n::ns) = insert n () (toNumSet ns)
+End
+
+Definition fromNumSet_def:
+  fromNumSet t = MAP FST (toAList t)
+End
+
+Definition mk_new_cutset_def:
+  mk_new_cutset ctxt (l:num_set) =
+    insert 0 () (toNumSet (MAP (find_var ctxt) (fromNumSet l)))
+End
+*)
+
+
+
+
+
+Definition compile_exp_def:
+  (compile_exp ctxt tmp l ((Const c):'a crepLang$exp) = (Skip, Const c, tmp, l)) /\
+  (compile_exp ctxt tmp l (Var v) = (Skip, Var (find_var ctxt v), tmp, l)) /\
+  (compile_exp ctxt tmp l (Label f) = (LocValue tmp (find_lab ctxt f), Var tmp, tmp + 1, l)) /\
+  (compile_exp ctxt tmp l (Load ad) =
+   let (p, le, tmp, l) = compile_exp ctxt tmp l ad in (p, Load le, tmp, l)) /\
+  (compile_exp ctxt tmp l (LoadByte ad) =
+   let (p, le, tmp, l) = compile_exp ctxt tmp l ad in
+    (Seq (Seq p (Assign tmp le)) (LoadByte tmp 0w tmp), Var tmp, tmp + 1, l)) /\
+  (compile_exp ctxt tmp l (LoadGlob gadr) = (Skip, Lookup gadr, tmp, l)) /\
+  (compile_exp ctxt tmp l (Op bop es) =
+   let (p, les, tmp, l) = compile_exps ctxt tmp l es in
+    (p, Op bop les, tmp, l)) /\
+  (compile_exp ctxt tmp l (Cmp cmp e e') =
+   let (p, le, tmp, l) = compile_exp ctxt tmp l e in
+   let (p', le', tmp', l) = compile_exp ctxt tmp l e' in
+    (prog_if cmp p p' le le' (tmp' + 1) (tmp' + 2) l, Var (tmp' + 1), tmp' + 3, insert (tmp' + 1) () l)) /\
+  (compile_exp ctxt tmp l (Shift sh e n) =
+   let (p, le, tmp, l) = compile_exp ctxt tmp l e in (p, Shift sh le n, tmp, l)) /\
+
+  (compile_exps ctxt tmp l cps = (* to generate ind thm *)
+   case cps of
+   | [] => (Skip, [], tmp, l)
+   | e::es =>
+     let (p, le, tmp, l) = compile_exp ctxt tmp l e in
+      let (p1, les, tmp, l) = compile_exps ctxt tmp l es in
+      (Seq p p1, le::les, tmp, l))
+Termination
+  cheat
+End
+
+ ‘es <> [] ==> MAP (EL 0) (MAP2 evals (comp_sts t ct tmp l es les) les) =
+    MAP (λe. eval r e) les’ by cheat >>
+   qpat_x_assum ‘word_op _ _ = _’ kall_tac >>
+   qpat_x_assum ‘EVERY _ _’ kall_tac >>
+   rpt (pop_assum mp_tac) >>
+   MAP_EVERY qid_spec_tac [‘t’, ‘p’, ‘les’ , ‘tmp’, ‘l’,‘ws’, ‘es’] >>
+   Induct
+   >- rw [] >>
+   rw [] >>
+   last_x_assum mp_tac >>
+   impl_tac >- metis_tac [] >>
+   fs [OPT_MMAP_def] >> rveq >>
+
+   fs [] >>
+
+
+Theorem bar:
+  !es ct tmp l.
+   ?les tmp' l'.
+   compile_exps ct tmp l es = (nested_seq (prog_comp ct tmp l es),les,tmp', l')
+
+    (le::les)  eval _ le = eval _ le
+
+
 Proof
-  rpt gen_tac >>
-  rpt strip_tac >>
-  fs [crepSemTheory.evaluate_def] >>
-  fs [CaseEq "option"] >> rveq >> fs [] >>
-  fs [compile_prog_def] >>
-  fs [evaluate_def] >>
+  Induct >> rw []
+  >- fs [compile_exp_def, nested_seq_def, prog_comp_def] >>
+  once_rewrite_tac [compile_exp_def] >>
+  fs [] >>
   pairarg_tac >> fs [] >>
-
-
-
-
+  pairarg_tac >> fs [] >>
+  fs [] >>
+  fs [prog_comp_def] >>
+  fs [nested_seq_def] >>
+  last_x_assum (qspecl_then [‘ct’, ‘tmp'’, ‘l'’] mp_tac) >>
+  fs []
 QED
 
+
+
+
+Definition temps_comp_def:
+  (temp_comp ct tmp l [] = [tmp]) /\
+  (temp_comp ct tmp l (e::es) = tmp ::
+   let (p, le, tmp, l) = compile_exp ct tmp l e in
+     temp_comp ct tmp l es)
+End
+
+
+Definition live_comp_def:
+  (live_comp ct tmp l [] = [l]) /\
+  (live_comp ct tmp l (e::es) = l ::
+   let (p, le, tmp, l) = compile_exp ct tmp l e in
+     live_comp ct tmp l es)
+End
+
+
+
+
+Definition eval_sts_def:
+  (eval_sts s [] = []) /\
+  (eval_sts s (p::ps) =
+   let (r,t) = evaluate (p,s) in
+     t :: eval_sts t ps)
+End
+
+Definition arrange_sts_def:
+  (arrange_sts sts [] = []) /\
+  (arrange_sts sts (le::les) =
+   TAKE (LENGTH (le::les)) sts ::
+    arrange_sts (DROP 1 sts) les)
+End
+
+
+Definition comp_sts_def:
+  comp_sts t ct tmp l es les =
+    arrange_sts (eval_sts t (prog_comp ct tmp l es)) les
+End
+
+
+Definition evals_def:
+  evals sts e = MAP (λst. eval st e) sts
+End
+
+(*
+Definition id_list_mem_def:
+  evals sts e = MAP (λst. eval st e) sts
+End
+*)
+
+
+(*
+Definition prog_if_def:
+  prog_if cmp p q e e' n m l =
+  nested_seq [
+    p; q;
+    Assign n e; Assign m e';
+    If cmp n (Reg m)
+    (Assign n (Const 1w)) (Assign n (Const 0w)) (insert n () l)]
+End
+
+Definition compile_exp_def:
+  (compile_exp ctxt tmp l ((Const c):'a crepLang$exp) = (Skip, Const c, tmp, l)) /\
+  (compile_exp ctxt tmp l (Var v) = (Skip, Var (find_var ctxt v), tmp, l)) /\
+  (compile_exp ctxt tmp l (Label f) = (LocValue tmp (find_lab ctxt f), Var tmp, tmp + 1, l)) /\
+  (compile_exp ctxt tmp l (Load ad) =
+   let (p, le, tmp, l) = compile_exp ctxt tmp l ad in (p, Load le, tmp, l)) /\
+  (compile_exp ctxt tmp l (LoadByte ad) =
+   let (p, le, tmp, l) = compile_exp ctxt tmp l ad in
+    (Seq (Seq p (Assign tmp le)) (LoadByte tmp 0w tmp), Var tmp, tmp + 1, l)) /\
+  (compile_exp ctxt tmp l (LoadGlob gadr) = (Skip, Lookup gadr, tmp, l)) /\
+  (compile_exp ctxt tmp l (Op bop es) =
+   let (p, les, tmp, l) = compile_exps ctxt tmp l es in
+    (nested_seq p, Op bop les, tmp, l)) /\
+  (compile_exp ctxt tmp l (Cmp cmp e e') =
+   let (p, le, tmp, l) = compile_exp ctxt tmp l e in
+   let (p', le', tmp', l) = compile_exp ctxt tmp l e' in
+    (prog_if cmp p p' le le' (tmp' + 1) (tmp' + 2) l, Var (tmp' + 1), tmp' + 3, insert (tmp' + 1) () l)) /\
+  (compile_exp ctxt tmp l (Shift sh e n) =
+   let (p, le, tmp, l) = compile_exp ctxt tmp l e in (p, Shift sh le n, tmp, l)) /\
+
+  (compile_exps ctxt tmp l cps = (* to generate ind thm *)
+   case cps of
+   | [] => ([Skip], [], tmp, l)
+   | e::es =>
+     let (p, le, tmp, l) = compile_exp ctxt tmp l e in
+      let (p1, les, tmp, l) = compile_exps ctxt tmp l es in
+      (p :: p1, le::les, tmp, l))
+Termination
+  cheat
+End
+
+
+Definition compile_prog_def:
+  (compile_prog _ l (Skip:'a crepLang$prog) = (Skip:'a loopLang$prog, l)) /\
+  (compile_prog ctxt l (Assign v e) =
+   case FLOOKUP ctxt.vars v of
+    | SOME n =>
+      let (p,le,tmp, l) = compile_exp ctxt (ctxt.vmax + 1) l e in (Seq p (Assign n le), l)
+    | NONE => (Skip,l))
+End
+
+ *) *)
 val _ = export_theory();
